feat: verified sponge_absorb (without unifying lemma)

lean/Shars/Verification/SpongeAbsorb.lean
@@ -12,110 +12,414 @@ import Shars.Verification.Utils
 import Shars.Verification.Refinement
 import Shars.Verification.Auxiliary
 import Shars.Verification.KeccakP
-import Shars.Verification.ListIR
+/- import Shars.Verification.ListIR -/
 
 set_option maxHeartbeats 100000
 attribute [-simp] List.getElem!_eq_getElem?_getD
 attribute [ext (iff := false)] List.ext_getElem!
 /- attribute [simp] Aeneas.Std.Slice.set -/
 
+theorem Spec.«toList_pad10*1»(x m: Nat)
+: let j := Int.toNat <| (- (m: Int) - 2) % x
+  (Spec.«pad10*1» x m).toList = [true] ++ List.replicate j false ++ [true]
+:= by simp [Spec.«pad10*1»]
+
+@[simp] theorem Spec.«pos_pad10*1»(x m: Nat)
+: (Spec.«pad10*1» x m).size > 0
+:= by simp [Spec.«pad10*1»]
+
 theorem getElem!_padding(x m: Nat)(i: Nat)
 : (Spec.«pad10*1» x m)[i]! = if i = 0 ∨ i = (Spec.«pad10*1» x m).size - 1 then true else false
 := by
-  split
-  case isTrue h =>
-    simp [Spec.«pad10*1»]
-    obtain h | h := h
-    · simp [h]; congr
-    · simp [h, Spec.«pad10*1»]; congr
-  case isFalse h =>
-    assume i_idx: i < (Spec.«pad10*1» x m).size
-    case otherwise => simp [getElem!_neg, i_idx]
-    simp [Spec.«pad10*1»] at h i_idx ⊢
-    simp_ifs
-    simp_lists
-    simp [default]
-
-theorem ref.mod_manipulation(a b r: Nat)
-  (h1: r ≥ 6)
-  (h2: a < r)
-  (h3: b <= 4)
-  (h4: (a + b) ≥ r)
-: ((- (a + b + 2: Int)) % r).toNat = 2*r - (a + b + 2)
-:= by
-  -- Big part of the equality
-  have: (((- (a + b + 2: Int)) % (r: Int))) = (2*r - (a + b + 2) ) % r := by
-    zmodify
+  rw [←Array.getElem!_toList, Spec.«toList_pad10*1»]
+  have pos := Spec.«pos_pad10*1» x m
+  assume i_idx: i < (Spec.«pad10*1» x m).size; case otherwise =>
+    rw [getElem!_neg]
     simp
-  rw [this]
-  -- Move equality to Int
-  zify
-  rw [Int.toNat_of_nonneg]
-  swap; {
-    apply Int.emod_nonneg
     omega
-  }
-  -- Show RHS is actually part of mod
-  rw [Int.emod_eq_of_lt]
-  · rw [Nat.cast_sub (by omega)]
-    zify
-  · omega
-  · omega
+    simp [Spec.«pad10*1»]at i_idx
+    scalar_tac
+  split
+  · rename_i h
+    obtain rfl | rfl := h
+    · simp
+    · simp [Spec.«pad10*1»]
+  · simp [Spec.«pad10*1»] at *
+    simp_lists
+
+/- theorem ref.mod_manipulation(a b r: Nat) -/
+/-   (h1: r ≥ 6) -/
+/-   (h2: a < r) -/
+/-   (h3: b <= 4) -/
+/-   (h4: (a + b) ≥ r) -/
+/- : ((- (a + b + 2: Int)) % r).toNat = 2*r - (a + b + 2) -/
+/- := by -/
+/-   -- Big part of the equality -/
+/-   have: (((- (a + b + 2: Int)) % (r: Int))) = (2*r - (a + b + 2) ) % r := by -/
+/-     zmodify -/
+/-     simp -/
+/-   rw [this] -/
+/-   -- Move equality to Int -/
+/-   zify -/
+/-   rw [Int.toNat_of_nonneg] -/
+/-   swap; { -/
+/-     apply Int.emod_nonneg -/
+/-     omega -/
+/-   } -/
+/-   -- Show RHS is actually part of mod -/
+/-   rw [Int.emod_eq_of_lt] -/
+/-   · rw [Nat.cast_sub (by omega)] -/
+/-     zify -/
+/-   · omega -/
+/-   · omega -/
 
 open Aeneas hiding Std.Array
 open Std.alloc.vec
 
-theorem Spec.«pad10*1_length» (x m : Nat)
-: (Spec.«pad10*1» x m).size = (2 + (-(m + 2: Int) % x).toNat)
-:= by simp +arith [«pad10*1», neg_add, -neg_add_rev, -Int.reduceNeg]
+def IR.absorb (s: List Bool) (chunks: List (List Bool)): List Bool := Id.run do
+  let mut s := s.setWidth (Spec.b 6)
+  for Pi in chunks do
+    s := IR.keccak_p (IR.xor s Pi)
+  return s
 
-def spec_sponge (r: Nat)(r_pos: r > 0):=
-  have: NeZero r := ⟨Nat.ne_zero_of_lt r_pos⟩
-  Spec.sponge (f := Spec.Keccak.P 6 24) (pad := Spec.«pad10*1»)
-def spec_sponge_absorb (r: Nat)(r_pos: r > 0) :=
-  have: NeZero r := ⟨Nat.ne_zero_of_lt r_pos⟩
-  Spec.sponge.absorb (f := Spec.Keccak.P 6 24) (pad := Spec.«pad10*1») (r := r)
-def spec_sponge_squeze{m d}(r: Nat)(r_pos: r > 0) :=
-  have: NeZero r := ⟨Nat.ne_zero_of_lt r_pos⟩
-  Spec.sponge.squeeze (m := m) (d := d) (f := Spec.Keccak.P 6 24) (r := r)
+@[simp] theorem Nat.mul_sub_successive(a b: Nat)
+: a * (b + 1) - a * b = a
+:= by simp only [Nat.mul_add, mul_one, add_tsub_cancel_left]
 
-/- #check BitVec.setWidth_cast -/
+-- #check List.extract
+-- theorem List.extract_append_drop_succ_eq_drop(ls: List α)(i n: Nat)
+--   (bnd: i + n ≤ ls.length)
+-- : ls.extract i (i + n) ++ ls.drop (i + n) = ls.drop i
+-- := by
+--   sorry
 
-def absorb.upd(S: BitVec (Spec.b 6))(P: Vector Bool r): BitVec (Spec.b 6) :=
-  Spec.Keccak.P 6 24 (S ^^^ (BitVec.ofBoolListLE <| P.toList).setWidth (Spec.b 6))
+theorem Spec.Keccak.toList_P(state: Spec.Bitstring (Spec.b 6))
+: (Keccak.P 6 24 state).toList = IR.keccak_p state.toList
+:= by simp [IR.keccak_p, List.toStateArray]
 
-def absorb{r: Nat}(S: BitVec (Spec.b 6))(Ps: Array (Vector Bool r)) := Id.run do
-  let mut S := S
-  for P in Ps do
-    S := absorb.upd S P
-  return S
+set_option maxHeartbeats 1000000 in
+@[progress]
+theorem algos.sponge_absorb_initial_loop.spec
+  (bs : Std.Slice Std.U8) (r : Std.Usize) (s : StateArray) (n i : Std.Usize)
+: n.val = bs.length / r.val
+→ (r_pos: r.val > 0)
+→ i.val ≤ n.val
+→ r.val < 200
+→ 8 ∣ r.val
+→ ∃ output,
+  sponge_absorb_initial_loop bs r s n i = .ok output ∧
+  output.toBits = IR.absorb s.toBits (bs.toBits.chunks_exact (8*r) |>.drop i)
+:= by
+  intro n_val r_pos i_idx r_le r_mtpl_8
+  unfold sponge_absorb_initial_loop
 
-def algos.sponge_absorb_final.panic_free
-  (keccak_p: List Bool → List Bool)
-  (r: Nat)
-  (s rest suffix: List Bool)
-: List Bool
-:= Id.run do
-  let mut s := s
-  s := ListIR.xor_long s rest
-  let nb_left := rest.length + suffix.length
-  if nb_left >= r then
-    s := ListIR.xor_long_at s (suffix.take (r - rest.length)) rest.length
-  -- if nb_left >= r then
-    s := keccak_p s
-    s := ListIR.xor_long s (suffix.drop (r - rest.length))
-    s := ListIR.xor_long_at s [true] (rest.length + suffix.length - r)
-    s := ListIR.xor_long_at s [true] (r-1)
-  else
-    s := ListIR.xor_long_at s suffix rest.length
-    s := ListIR.xor_long_at s [true] nb_left
-    if nb_left + 1 < r then
-      s := ListIR.xor_long_at s [true] (r-1)
+   -- r * (i + 1) ≤ r * n = r * (bs.length / r) ≤ bs.length            ( ≤ Usize.max )
+  have r_range(i_idx: i < n): r.val*i.val + r.val ≤ bs.length := calc r.val * i.val + r.val
+      _ ≤ r.val * n := Nat.mul_le_mul_left r.val i_idx
+      _ = r.val * (bs.length / r) := by simp [n_val]
+      _ ≤ bs.length := Nat.mul_div_le bs.length ↑r
+
+  progress*
+  · simp [*, IR.absorb, Nat.mul_add, Spec.Keccak.toList_P]
+    simp [*] at chunk_post
+    rw [←List.getElem_cons_drop_succ_eq_drop (i := i)]
+    swap; { simp +arith [Nat.mul_div_mul_left]; scalar_tac}
+    simp +decide [-List.getElem_cons_drop, Std.Array.toBits, List.toStateArray]
+    congr
+    simp [*, Std.Slice.toBits, ←getElem!_pos,]
+    rw [List.getElem!_chunks_exact]; case a => simp +arith [Nat.mul_div_mul_left]; scalar_tac
+    simp
+    ring_nf
+
+  case isFalse i_oob =>
+    have := ‹bs.length / r.val - i.val = 0›'
+    simp [IR.absorb, this]
+    rw [List.drop_of_length_le ?bnd]; case bnd => simp +arith [Nat.mul_div_mul_left]; scalar_tac
+    simp +decide [Std.Array.toBits, List.setWidth_of_length_eq]
+termination_by n.val - i.val
+decreasing_by scalar_decr_tac
+
+@[progress]
+theorem algos.sponge_absorb_initial.spec
+  (bs : Std.Slice Std.U8) (r : Std.Usize) (s : StateArray)
+: (r_pos: r.val > 0)
+→ r.val < 200
+→ 8 ∣ r.val
+→ ∃ output,
+  sponge_absorb_initial bs r s = .ok output ∧
+  output.toBits = IR.absorb s.toBits (bs.toBits.chunks_exact (8*r))
+:= by intros
+      unfold sponge_absorb_initial
+      progress*
+      simp [*]
+
+theorem Vector.append_cast(b1: Vector α n)(b2: Vector α m)
+  (h1: n = n')(h2: m = m')
+: b1.cast h1 ++ b2.cast h2 = (b1 ++ b2).cast (show n + m = n' + m' from by simp [h1, h2])
+:= by ext i i_idx; by_cases i < n <;> simp [h1 ▸ i_idx, *, Vector.getElem_append]
+
+theorem Vector.append_cast_left(b1: Vector α n)(b2: Vector α m)
+  (h: n = n')
+: b1.cast h ++ b2 = (b1 ++ b2).cast (show n + m = n' + m from by simp [h])
+:= by rw [←Vector.cast_rfl (n := m) (xs := b2)]; apply Vector.append_cast
+
+theorem Vector.append_cast_right(b1: Vector α n)(b2: Vector α m)
+  (h: m = m')
+: b1 ++ b2.cast h = (b1 ++ b2).cast (show n + m = n + m' from by simp [h])
+:= by rw [←Vector.cast_rfl (n := n) (xs := b1)]; apply Vector.append_cast
+
+
+def IR.array_absorb.upd (r: Nat) (r_bnd: r < Spec.b 6) (state : Spec.Bitstring (Spec.b 6)) (chunk : Vector Spec.Bit r) :=
+   Spec.Keccak.P 6 24 (state ^^^ (chunk ++ Vector.replicate (Spec.b 6 - r) false).cast (by simp [*, le_of_lt]))
+
+def IR.array_absorb(r: Nat)(r_bnd: r < Spec.b 6)(arr: Array (Spec.Bitstring r))
+  (init: Spec.Bitstring (Spec.b 6) := Vector.replicate (Spec.b 6) false)(i: Nat := 0)
+:= arr.toList.drop i |>.foldl (IR.array_absorb.upd r r_bnd) init
+
+def IR.array_absorb.refinement(r: Nat)(r_pos: r > 0)(r_bnd: r < Spec.b 6)(N: Array Spec.Bit)
+: Spec.sponge.absorb (f := Spec.Keccak.P 6 24) (pad := Spec.«pad10*1») (r := ⟨r, ⟨r_pos, r_bnd⟩⟩) N = IR.array_absorb r r_bnd (Array.chunks_exact r (N ++ Spec.«pad10*1» r N.size))
+:= by
+  unfold Spec.sponge.absorb IR.array_absorb IR.array_absorb.upd
+  simp [*, Vector.setWidth, Vector.append_cast_left]
+
+def IR.array_absorb.unfold(r: Nat)(r_bnd: r < Spec.b 6)(arr: Array (Spec.Bitstring r))(i: Nat)
+: IR.array_absorb r r_bnd arr init i =
+    if i < arr.size then
+      let init := IR.array_absorb.upd r r_bnd init arr[i]!
+      IR.array_absorb r r_bnd arr init (i + 1)
     else
-      s := keccak_p s
-      s := ListIR.xor_long_at s [true] (r-1)
-  keccak_p s
+      init
+:= by
+  simp [IR.array_absorb]
+  by_cases h: i < arr.size
+  · simp [*]
+    rw [←List.getElem_cons_drop h]
+    simp [←getElem!_pos]
+  · simp [*, ←getElem!_pos, List.drop_of_length_le, not_lt.mp]
 
+def IR.absorb.loop (s: List Bool) (chunks: List (List Bool))(i: Nat := 0): List Bool := Id.run do
+  let mut s := s.setWidth (Spec.b 6)
+  for Pi in chunks.drop i do
+    s := IR.keccak_p (IR.xor s Pi)
+  return s
+
+def IR.absorb.unfold(s: List Bool)(chunks: List (List Bool))
+: IR.absorb s chunks = IR.absorb.loop s chunks
+:= by simp only [absorb, loop, List.drop_zero]
+
+def IR.absorb.loop.unfold(init: List Bool)(chunks: List (List Bool))(i: Nat)
+: IR.absorb.loop init chunks i =
+    let init := (init.setWidth (Spec.b 6))
+    if i < chunks.length then
+      let init := IR.keccak_p (IR.xor init chunks[i]!)
+      IR.absorb.loop init chunks (i + 1)
+    else
+      init
+:= by
+  simp [loop]
+  by_cases h: i < chunks.length
+  · simp [*]
+    rw [←List.getElem_cons_drop h]
+    simp [←getElem!_pos]
+  · simp [*, List.drop_of_length_le, not_lt.mp]
+
+theorem Vector.toList_xor(b1 b2: Vector Bool n)
+: (b1 ^^^ b2).toList = IR.xor b1.toList b2.toList
+:= by
+  apply List.ext_getElem
+  · simp
+  simp [←getElem!_pos]
+  intro i i_idx
+  simp [HXor.hXor, Xor.xor, Vector.getElem!_ofFn, i_idx, ←getElem!_pos]
+  simp [IR.xor, i_idx, List.getElem!_zipWith]
+
+@[simp]
+theorem IR.xor_zero(state: List Bool)
+: IR.xor state (List.replicate n false) = state
+:= by
+  apply List.ext_getElem <;> simp [←getElem!_pos]
+  intro i i_idx
+  unfold IR.xor
+  by_cases cond: i < n
+  · simp [*, List.getElem!_append_left, List.getElem!_zipWith]
+  · simp [*, not_lt.mp, List.getElem!_append_right]; congr; omega
+
+set_option maxHeartbeats 1000000 in
+@[simp]
+theorem IR.xor_append(state: List Bool)
+: IR.xor state (bs1 ++ bs2) = IR.xor (IR.xor state  bs1) (List.replicate bs1.length false ++ bs2)
+:= by
+  apply List.ext_getElem <;> simp [←getElem!_pos]
+  intro i i_idx
+  unfold IR.xor
+  if left: i < bs1.length then
+    simp_lists
+    simp
+  else if right: i < bs2.length then
+    simp_lists
+    simp
+  else
+    simp_lists
+    simp
+
+theorem IR.absorb.refinement  (r: Nat)(r_pos: r > 0)(r_bnd: 8*r < Spec.b 6)(chunks : Array (Spec.Bitstring (8*r)))(init: Spec.Bitstring (Spec.b 6))(i: Nat)
+: (array_absorb (8 * r) r_bnd chunks init i).toList = IR.absorb.loop init.toList (chunks.toList.map (·.toList)) i
+:= by
+  rw [IR.array_absorb.unfold]
+  rw [IR.absorb.loop.unfold]
+  simp
+  if cond: i < chunks.size then
+    simp [cond, IR.array_absorb.upd]
+    rw [IR.absorb.refinement r r_pos r_bnd]
+    simp [Spec.Keccak.toList_P]
+    simp [Vector.toList_xor]
+  else
+    simp [cond]
+
+attribute [simp_scalar_simps] Nat.add_sub_cancel
+
+attribute [-simp] Bool.if_false_right Bool.if_false_left Bool.if_true_right Bool.if_true_left IR.xor_append in
+set_option maxHeartbeats 1000000 in
+@[progress]
+theorem algos.sponge_absorb_final.spec
+  (input : StateArray) (rest : Std.Slice Std.U8) (extra : Std.U8) (r : Std.Usize)
+: r.val ≥ 6
+→ r.val ≤ 200
+→ rest.length < r
+→ extra.toBits[7]! = false
+→ ∃ output,
+  sponge_absorb_final input rest extra r = .ok output ∧
+  output.toBits = IR.absorb input.toBits [rest.toBits ++ (extra.toBits.setWidth (8*r- 8*rest.length - 1)) ++ [true]]
+:= by
+  intro r_big_enough r_bnd length_rest_lt extra_padding_no_collision
+  unfold sponge_absorb_final
+  progress*
+  simp [*, Std.Array.toBits, IR.absorb, IR.keccak_p]
+  congr 3
+  apply List.ext_getElem
+  · simp +decide
+  simp +decide [←getElem!_pos]
+
+  have: 128#u8.toBits = List.replicate 7 false ++ [true] := by decide
+  simp only [this, List.replicate_append_replicate, ←List.append_assoc, Nat.mul_sub, ‹8*r.val - 8 + 7 = 8*r.val - 1›']
+  /-
+
+  +────────────────────────────────────────────────────────────+
+  |                    input                                   |
+  +────────────────────────────────────────────────────────────+
+                                                               ↑
+  +─────────────────+────────────+                             |
+  |       rest      |   extra    |                             |
+  +─────────────────+────────────+                             |
+                                                               |
+                    +────────────────────────────+             |
+                    |···························1|             |
+                    +────────────────────────────+             |
+                    ↑                          ↑ ↑             |
+                    |                          | |             |
+                    rest.length                | r             1600
+                                              r-1
+  -/
+  intro i i_idx
+  simp [IR.xor_assoc, IR.getElem!_xor, i_idx]
+  rw [(show input.val.toBits[i]! = (input.val.toBits[i]! ^^ false) from by simp)]
+  simp only [Bool.xor_assoc]
+  rw [←apply_ite (f := (fun (x: Bool) => input.val.toBits[i]! ^^ x))]
+  simp only [Bool.false_bne, Bool.bne_right_inj]
+
+  -- TODO: I would like `simp_scalar` to do all of this.
+  rw [Nat.sub_add_cancel]; swap; { scalar_tac}
+  rw [←Nat.mul_comm 8]
+  rw [Nat.sub_add_cancel]; swap; { scalar_tac}
+  rw [←Nat.add_sub_assoc]; swap; { scalar_tac}
+  simp
+
+  if i < 8*rest.length then
+    simp_ifs
+    simp_lists
+    simp
+  else if i < 8*r.val - 1 then
+    simp_ifs
+    simp_lists
+    simp [Std.UScalar.getElem!_toBits, ←Nat.mul_comm 8]
+    simp_ifs
+  else if i < 8*r.val then
+    simp [*, ‹i = 8*r - 1›']
+    simp_ifs
+    simp_lists
+    if rest.length = r - 1 then
+      simp [*, Nat.mul_sub, ‹8*r.val - 1 - (8*r.val - 8) = 7›']
+    else
+      rw [getElem!_neg]; case h => simp [Std.UScalar.length_toBits]; scalar_tac
+      simp
+  else
+    simp_ifs
+    simp_lists
+    rw [getElem!_neg]
+    case h => simp; scalar_tac
+    simp
+
+attribute [scalar_tac_simps] Nat.div_mul_le_self Nat.mul_div_le
+
+@[simp]
+theorem IR.length_absorb_loop(s: List Bool)(bs: List (List Bool))(i: Nat)
+: (absorb.loop s bs i).length = Spec.b 6
+:= by
+  rw [absorb.loop.unfold]
+  by_cases i < bs.length <;> simp [*]
+  rw [IR.length_absorb_loop]
+
+@[simp]
+theorem IR.absorb_absorb(s: List Bool)(bs bs2: List (List Bool))
+: absorb (absorb s bs) bs2 = absorb s (bs ++ bs2)
+:= by
+  simp only [absorb.unfold]
+  have len_absorb := IR.length_absorb_loop s bs 0
+  simp [absorb.loop] at *
+  rw [List.setWidth_of_length_eq]
+  simpa using len_absorb
+
+theorem Array.toList_chunks_exact(arr: Array α)(r: Nat)
+: (arr.chunks_exact r).toList.map (·.toList) = arr.toList.chunks_exact r
+:= by
+  obtain ⟨data⟩ := arr
+  if r_pos: r = 0 then
+    subst r_pos
+    simp [chunks_exact, List.chunks_exact]
+  else if data_small: data.length < r then
+    unfold chunks_exact List.chunks_exact
+    simp [Nat.le_of_sub_eq_zero, Nat.lt_of_add_one_le, *]
+  else
+    have: data.length ≥ r := by omega
+    unfold chunks_exact List.chunks_exact
+    simp [*, not_lt.mpr]
+    rw [Array.toList_chunks_exact]
+    simp [List.take_of_length_le]
+termination_by arr.size + 1 - r
+decreasing_by simp [*]; omega
+
+theorem List.chunks_exact_truncate{α: Type}(bs: List α)(r: Nat)
+: (bs.take (r*(bs.length/r))).chunks_exact r = bs.chunks_exact r
+:= by
+  assume r_pos: r > 0
+  case otherwise => simp at r_pos; subst r_pos; simp [List.chunks_exact]
+  have r_neZero: NeZero r := NeZero.of_pos r_pos
+  cases bs using List.cases_extract r
+  case onSmall small =>
+    unfold List.chunks_exact
+    simp [*]
+  case onBig chunk rest len_chunk =>
+    unfold List.chunks_exact
+    simp [*, r_neZero.out]
+    have: r <= r*(rest.length / r + 1) := by ring_nf; simp
+    have: rest.length / r + 1 = (chunk ++ rest).length / r := by simp [len_chunk, Nat.add_div_left, r_pos]
+    simp_lists [len_chunk]
+    simp +arith
+    ring_nf
+    simp +arith
+    apply List.chunks_exact_truncate
+termination_by bs.length
+decreasing_by simp [*]
 
 @[scalar_tac_simps]
 theorem Nat.sub_div_self(a b: Nat)
@@ -143,800 +447,1041 @@ theorem Nat.sub_div_mult_left(a b: Nat)
       simp [Nat.mul_add, Nat.sub_add_eq, Nat.sub_div_self]
       rw [Nat.sub_div_mult_left]
 
-theorem BitVec.cast_xor(bv bv2: BitVec n)(eq: n = m)
-: (bv ^^^ bv2).cast eq = bv.cast eq ^^^ bv2.cast eq
-:= by ext i i_lt; simp
 
-attribute [simp] Aeneas.Std.core.slice.index.Slice.index
-
-
-private theorem List.foldl_congr{ls ls': List α}
-: ls = ls'
-→ upd = upd'
-→ init = init'
-→ ls.foldl upd init = ls'.foldl upd' init'
-:= by rintro rfl rfl rfl; rfl
-
-set_option trace.SimpIfs true in
-set_option maxRecDepth 1000000 in
-set_option maxHeartbeats 1000000 in
-theorem absorb.refinement(r: Nat)(S: BitVec (Spec.b 6))(bs: Array Bool)
-: (absorb S (bs.chunks_exact r)).toList = ListIR.absorb' ListIR.list_keccak_p S.toList (bs.toList.chunks_exact r)
-:= by
-  unfold absorb ListIR.absorb'
-  simp [ListIR.list_keccak_p, ListIR.xor_long.def, -Array.size_chunks_exact]
-  rw [←Array.foldl_toList]
-  rw [Array.chunks_exact, List.chunks_exact]
-  split <;> simp_ifs
-  case isTrue h =>
-    simp
-    ext i
-    · simp [Spec.b, Spec.w]
-    by_cases i < 1600 <;> simp
-    case pos h => intros; assumption
-    case neg h =>
-      rw [getElem!_neg]
-      case h => simpa using h
-      simp
-  case isFalse h =>
-    simp
-    generalize_proofs _ len_extract
-    have ih := absorb.refinement r (@upd r S ⟨bs.extract 0 r, len_extract⟩) (bs.extract r)
-    simp [absorb,ListIR.absorb', ListIR.list_keccak_p, ListIR.xor_long.def] at ih
-    rw [ih]
-    rw [List.foldl_congr]
-    · rw [List.take_of_length_le]
-      simp
-    · ext s chunk
-      · simp
-      simp
-    · rw [upd]
-      simp [List.setWidth, Spec.b, Spec.w]
-      rw [List.take_of_length_le (by simp)]
-      apply congrArg
-      apply congrArg
-      ext i i_idx
-      rw [ListIR.xor_long, ListIR.xor_long_at]
-      simp at i_idx
-      simp [←Bool.default_bool,←List.getElem!_eq_getElem?_getD, i_idx]
-      have: S.toList.length = 1600 := by simp [Spec.b, Spec.w]
-      if h: i < r then
-        simp_lists
-        rw [List.getElem!_zipWith]
-        case a => simp [*]
-        case a => simp [*]; omega
-        simp [getElem_eq_getElem!, *]
-      else
-        simp_lists
-        simp at h
-        simp +arith [getElem_eq_getElem!, ←Nat.add_sub_assoc, h]
-termination_by bs.size
-
-abbrev ref.interesting_part_of_the_proof.preconditions(r: Nat)(s rest suffix: List Bool) :=
-  r ≥ 6 -- Otherwise, we don't have suffix + 2 ≤ r
-∧ suffix.length ≤ 4 -- Taken from the actual uses of `suffix` in SHA3
-∧   rest.length < r -- Since rest is what's left after absorb_initial
-∧ s.length = 1600 -- The state has length Spec.b 6
-
-set_option maxRecDepth 100000000 in
-set_option maxHeartbeats 1000000 in
-theorem ref.interesting_part_of_the_proof.case1{r: Nat}{s rest suffix: List Bool}
-  (hyp: (rest ++ suffix).length ≥ r)
-: preconditions r s rest suffix
-→ let padding := (Spec.«pad10*1» r (rest.length + suffix.length)).toList
-  (rest ++ suffix ++ padding).chunks_exact r = [(rest ++ suffix).take r, (suffix.drop (r - rest.length) ++ padding)]
-:= by
-  /-
-  · (rest ++ suffix) >= r
-    Then we have
-     (rest ++ suffix ++ padding).chunks_exact k =
-     = [(rest ++ suffix).take r, (suffix.drop (r - rest.length) ++ padding)]
-  -/
-  rintro ⟨r_big_enough,suffix_len_le,rest_len_lt,len_s⟩ padding
-  have len_padding: (Spec.«pad10*1» r (rest.length + suffix.length)).size = 2*r - (rest.length + suffix.length) := by
-    simp [Spec.«pad10*1_length», -neg_add_rev]
-    have := mod_manipulation (h1 := r_big_enough) (h2 := rest_len_lt) (h3 := suffix_len_le) (h4 := by scalar_tac)
-    rw [this]
-    scalar_tac
-  have len_append: (rest.length + suffix.length + padding.length) = 2*r := by
-    simp [padding, len_padding]
-    scalar_tac
-  simp at hyp
-  have len_chunks: ((rest ++ suffix ++ padding).chunks_exact r).length = 2 := by
-    simp
-    rw [←Nat.add_assoc, len_append, Nat.mul_div_cancel]
-    omega
-
-  -- Execute List.chunks_exact
-  unfold List.chunks_exact
-  simp_ifs
-  unfold List.chunks_exact
-  simp_ifs
-  unfold List.chunks_exact
-  simp_ifs
-
-  congr 1
-  · ext i
-    · simp [←Nat.add_assoc, len_append]
-      omega
-    by_cases i < r
-    case neg => simp_lists
-    rw [List.getElem!_take_append_beg]
-    case pos.x => assumption
-    case pos.x => simp; omega
-    simp_lists
-  · congr
-    ext i
-    · simp [←Nat.add_assoc, len_append]
-      omega
-    simp_lists
-    congr
-    omega
-
-set_option maxRecDepth 100000000 in
-set_option maxHeartbeats 1000000 in
-theorem ref.interesting_part_of_the_proof.case2{r: Nat}{s rest suffix: List Bool}
-  (hyp: (rest ++ suffix).length = r-1)
-: preconditions r s rest suffix
-→ let padding := (Spec.«pad10*1» r (rest.length + suffix.length)).toList
-  (rest ++ suffix ++ padding).chunks_exact r = [rest ++ suffix ++ [true], List.replicate (r-1) false ++ [true]]
-:= by
-  /-
-  · (rest ++ suffix) = r - 1
-    Then we have
-     (rest ++ suffix ++ padding).chunks_exact k =
-     = [rest ++ suffix ++ [true], List.replicate false (r-1) ++ [true]]
-  -/
-  rintro ⟨r_big_enough,suffix_len_le,rest_len_lt,len_s⟩ padding
-  have len_padding: (Spec.«pad10*1» r (rest.length + suffix.length)).size = 2*r - (rest.length + suffix.length) := by
-    simp at hyp
-    simp [Spec.«pad10*1_length», -neg_add_rev, hyp, r_big_enough]
-    zify
-    rw [Nat.cast_sub (by omega)]
-    rw [Nat.cast_sub (by omega)]
-    rw [Nat.cast_sub (by omega)]
-    rw [Nat.cast_mul]
-    ring_nf
-    simp [Int.neg_emod_eq_sub_emod]
-    rw [
-      Int.emod_eq_of_lt (H1:=by omega) (H2:=by omega),
-      Int.max_eq_left (by omega)
-    ]
-    omega
-  have len_append: (rest.length + suffix.length + padding.length) = 2*r := by
-    simp [padding, len_padding]; scalar_tac
-
-  simp at hyp
-  have len_chunks: ((rest ++ suffix ++ padding).chunks_exact r).length = 2 := by
-    simp
-    rw [←Nat.add_assoc, len_append, Nat.mul_div_cancel]
-    omega
-
-  -- Execute List.chunks_exact
-  unfold List.chunks_exact
-  simp_ifs
-  unfold List.chunks_exact
-  simp_ifs
-  unfold List.chunks_exact
-  simp_ifs
-  congr
-  · ext i
-    · simp; scalar_tac
-    simp_lists
-    congr
-    simp [hyp, Nat.sub_sub_self, ‹r >= 1›', List.take_one, List.head?, padding, Spec.«pad10*1», BitVec.toList]
-  · ext i
-    · simp; scalar_tac
-    simp_lists
-    simp [hyp] at len_padding
-    simp [hyp, Nat.sub_sub_self, ‹r >= 1›', padding, Array.getElem!_toList, getElem!_padding, len_padding,
-       -Bool.if_false_right, -Bool.if_false_left, -Bool.if_true_left] -- Keep `if`s for `simp_ifs` to process
-    by_cases i = r -1
-    case pos h => simp_ifs [h]; simp
-    case neg =>
-      simp_ifs
-      by_cases i > r - 1
-      case neg => simp_ifs
-      case pos =>
-        simp_ifs
-        rw [getElem!_neg]
-        simp
-        scalar_tac
-
-set_option maxRecDepth 100000000 in
-set_option maxHeartbeats 1000000 in
-theorem ref.interesting_part_of_the_proof.case3{r: Nat}{s rest suffix: List Bool}
-  (hyp: (rest ++ suffix).length <= r-2)
-: preconditions r s rest suffix
-→ let padding := (Spec.«pad10*1» r (rest.length + suffix.length)).toList
-  (rest ++ suffix ++ padding).chunks_exact r = [rest ++ suffix ++ [true] ++ List.replicate (r -2 - rest.length - suffix.length) false ++ [true]]
-:= by
-  /-
-  · (rest ++ suffix) <= r - 2
-    Then we have
-     (rest ++ suffix ++ padding).chunks_exact k =
-     = [rest ++ suffix ++ [true, true]]
-  -/
-  rintro ⟨r_big_enough,suffix_len_le,rest_len_lt,len_s⟩ padding
-  have len_padding: (Spec.«pad10*1» r (rest.length + suffix.length)).size = r - (rest.length + suffix.length) := by
-    simp at hyp
-    simp [Spec.«pad10*1_length», -neg_add_rev]
-    zify
-    rw [Nat.cast_sub (by omega),
-        Int.neg_emod_eq_sub_emod,
-        Int.emod_eq_of_lt (H1:=by omega) (H2:=by omega)]
-    simp
-    rw [Int.max_eq_left (by omega)]
-    omega
-  have len_append: (rest.length + suffix.length + padding.length) = r := by
-    simp [padding, len_padding]
-    scalar_tac
-  have len_chunks: ((rest ++ suffix ++ padding).chunks_exact r).length = 1 := by
-    simp [←Nat.add_assoc, len_append, Nat.div_self, ‹r > 0›']
-
-  unfold List.chunks_exact
-  simp_ifs
-
-  unfold List.chunks_exact
-  simp_ifs
-  simp
-  ext i
-  · simp; scalar_tac
-  simp_lists
-  congr
-  simp [padding, Spec.«pad10*1», BitVec.toList]
-  have := Spec.«pad10*1_length» r (rest.length + suffix.length)
-  simp at this
-  ring_nf at this ⊢
-  scalar_tac
-
-set_option maxHeartbeats 1000000 in
-theorem ref.interesting_part_of_the_proof.proof(r: Nat)(s rest suffix: List Bool)
-: preconditions r s rest suffix
-→ let f := ListIR.list_keccak_p
-  let padding := (Spec.«pad10*1» r (rest.length + suffix.length)).toList
-  algos.sponge_absorb_final.panic_free f r s rest suffix =
-    ListIR.absorb' f s (
-      (rest ++ suffix ++ padding).chunks_exact r
-    )
-:= by
-  rintro precond f padding
-  have ⟨r_big_enough,suffix_len_le,rest_len_lt,len_s⟩ := precond
-  /-
-  There are three cases we must consider:
-  · (rest ++ suffix) >= r
-    Then we have
-     (rest ++ suffix ++ padding).chunks_exact k =
-     = [(rest ++ suffix).take r, (suffix.drop (r - rest.length) ++ padding)]
-  · (rest ++ suffix) = r - 1
-    Then we have
-     (rest ++ suffix ++ padding).chunks_exact k =
-     = [rest ++ suffix ++ [true], List.replicate false (r-1) ++ [true]]
-  · (rest ++ suffix) <= r - 2
-    Then we have
-     (rest ++ suffix ++ padding).chunks_exact k =
-     = [rest ++ suffix ++ [true, true]]
-  -/
-  if      cond1: (rest ++ suffix).length ≥ r then
-    rw [case1 cond1 precond]
-    simp at cond1
-    simp [ListIR.absorb', algos.sponge_absorb_final.panic_free, *, ListIR.xor_long]
-
-    generalize leftover_val: (rest.length + suffix.length - r) = leftover
-    rw [ListIR.xor_long_at_twice_separate]
-    case compatible_offset => scalar_tac
-
-    rw [ListIR.xor_long_at_twice_separate]
-    case compatible_offset => scalar_tac
-
-    rw [ListIR.xor_long_at_twice_separate]
-    case compatible_offset => scalar_tac
-
-    congr
-    · simp +arith [List.take_append_of_ge_length, le_of_lt rest_len_lt]
-    · simp +arith; scalar_tac
-    · have padding_len
-      : (Spec.«pad10*1» r (rest.length + suffix.length)).size = 2 * r - rest.length - suffix.length
-      := by
-        simp [Spec.«pad10*1»]
-        have: (2: Int) = (2: Nat).cast := by congr
-        rw [this]
-        have(a b: Int): a - b = a + -b := by exact rfl
-        rw [this]
-        simp only [←Nat.cast_sub, ←neg_add, Nat.cast_add]
-        conv =>
-          lhs
-          rhs
-          rw [Nat.cast_ofNat]
-          conv => enter [1, 1, 1, 1, 1]; rw [Int.add_comm]
-          rw [mod_manipulation (h1 := r_big_enough) (h2 := rest_len_lt) (h3 := suffix_len_le) (h4 := cond1)]
-        scalar_tac
-
-      ext i
-      · simp [padding_len]
-        scalar_tac
-      conv => rhs; rw [Array.getElem!_toList]
-      simp [getElem!_padding, -List.cons_append, -List.singleton_append, -List.cons_append_fun]
-      by_cases h: i = 0
-      case pos => simp [h]
-      by_cases h: i = (Spec.«pad10*1» r (rest.length + suffix.length)).size - 1
-      -- by_cases h: i = 2* r - rest.length - suffix.length - 1
-      case pos =>
-        rw [List.getElem!_append_right]
-        case h => scalar_tac
-        rw [List.getElem!_append_right]
-        case h => scalar_tac
-        simp [h, padding_len, ←leftover_val]
-        rw [List.getElem!_singleton]
-        scalar_tac
-      by_cases h: i < (Spec.«pad10*1» r (rest.length + suffix.length)).size
-      case neg =>
-        rw [getElem!_neg]
-        case h => simp [Spec.«pad10*1»] at *; scalar_tac
-        simp [Spec.«pad10*1»] at *
-        simp [*]
-      case pos =>
-        rw [getElem!_pos]
-        case h => simp [padding_len] at *; scalar_tac
-        rw [List.getElem_append_right]
-        case h₁ => scalar_tac
-        rw [List.getElem_append_left]
-        case h => scalar_tac
-        simp [padding_len] at *; simp [*]
-        scalar_tac
-
-  else if cond2: (rest ++ suffix).length = r - 1 then
-    rw [case2 cond2 precond]
-    replace cond2 := ‹r = (rest ++ suffix).length + 1›'
-    simp [ListIR.absorb', algos.sponge_absorb_final.panic_free, *, ListIR.xor_long]
-
-    rw [ListIR.xor_long_at_twice_separate]
-    case compatible_offset => scalar_tac
-
-    rw [ListIR.xor_long_at_twice_separate]
-    case compatible_offset => scalar_tac
-
-    simp [ListIR.xor_long_of_xor_long_at]
-    congr
-    -- have{α: Type}(x ls: List α): (x ++ ls) = ls ↔ x = [] := by exact?
-    simp_lists
-    scalar_tac
-
-  else if cond3: (rest ++ suffix).length ≤ r - 2 then
-    rw [case3 cond3 precond]
-    simp at cond3
-    simp [ListIR.absorb', algos.sponge_absorb_final.panic_free, *, ListIR.xor_long]
-    simp_ifs
-
-    rw [ListIR.xor_long_at_twice_separate]
-    case compatible_offset => scalar_tac
-
-    rw [ListIR.xor_long_at_twice_separate]
-    case compatible_offset => scalar_tac
-
-    rw [ListIR.xor_long_at_twice_separate]
-    case compatible_offset => scalar_tac
-
-    simp only [ListIR.xor_long_of_xor_long_at]
-    congr
-    · simp
-    · rw [List.append_right_eq_self, List.replicate_eq_nil_iff]
-      -- scalar_tac -- TODO: Gives maxRecDepth error
-      omega
-    · simp only [List.length_singleton, Nat.sub_add_eq]
-      congr
-
-  else omega -- Absurd
-
-theorem absorb_def{r: Nat}(S: BitVec (Spec.b 6))(Ps: Array (Vector Bool r))
-: absorb S Ps = Ps.foldl (absorb.upd · ·) S
-:= by simp [absorb]
-
-theorem absorb.spec (N : Array Spec.Bit) (r: Nat)(r_pos: r > 0)
-: spec_sponge_absorb r r_pos N = absorb (0#(Spec.b 6)) ((N ++ Spec.«pad10*1» r N.size).chunks_exact r)
-:= by
-  rw [spec_sponge_absorb, Spec.sponge.absorb, absorb]
-  -- NOTE: I needed to exercise a bit too much control here.
-  simp [←Array.foldl_toList,-Array.size_chunks_exact, -Array.size_map, upd]
-
-@[progress]
-theorem Aeneas.Std.Array.to_slice_mut.spec{α : Type u} {n : Usize} (a : Array α n)
-: ∃ old new,
-  Std.toResult (a.to_slice_mut) = .ok (old, new) ∧
-  old = a.to_slice ∧
-  new = a.from_slice
-:= by simp [to_slice_mut, Std.toResult]
-
-attribute [simp] Std.Slice
-set_option maxHeartbeats 1000000 in
-@[progress]
-theorem algos.sponge_absorb_initial_loop.spec
-  (bs : Std.Slice Bool) (r : Std.Usize) (s : Aeneas.Std.Array Bool 1600#usize) (n i : Std.Usize)
-: n.val = bs.length / r.val
-→ (r_pos: r.val > 0)
-→ i.val ≤ n.val
-→ r.val < 1600
-→ ∃ output,
-  sponge_absorb_initial_loop bs r s n i = .ok output ∧
-  output.val.toBitVec = (
-    (
-      absorb (s.val.toBitVec.cast (by simp [Spec.w, Spec.b])) (bs.val.toArray.chunks_exact r |>.drop i)
-    ).cast (by simp [Spec.w, Spec.b])
-  )
-:= by
-  rintro n_val r_pos i_idx r_le
-  rw [sponge_absorb_initial_loop]
-  split
-  case isTrue i_idx =>
-     -- r * i < r * n = r * (bs.length / r) ≤ bs.length ≤ Usize.max
-    have _: r.val*i.val ≤ bs.length := le_of_lt $ calc r.val * i.val
-        _ < r.val * n := Nat.mul_lt_mul_of_pos_left i_idx r_pos
-        _ = r.val * (bs.length / r) := by simp [n_val]
-        _ ≤ bs.length := Nat.mul_div_le bs.length ↑r
-
-     -- r * (i + 1) ≤ r * n = r * (bs.length / r) ≤ bs.length ≤ Usize.max
-    have _: r.val*(i.val + 1) ≤ bs.length := calc r.val * (i.val + 1)
-        _ ≤ r.val * n := Nat.mul_le_mul_left r.val i_idx
-        _ = r.val * (bs.length / r) := by simp [n_val]
-        _ ≤ bs.length := Nat.mul_div_le bs.length ↑r
-
-    let* ⟨ i1, i1_post ⟩ ← Std.Usize.mul_spec
-    let* ⟨ i2, i2_post ⟩ ← Std.Usize.add_spec
-    let* ⟨ i3, i3_post ⟩ ← Std.Usize.mul_spec
-    let* ⟨ slice, slice_post ⟩ ← Std.core.slice.index.Slice.index.slice_index_range_usize_slice_spec
-    fsimp only [*] at slice_post
-    let* ⟨old_slice, new_slice, slice_mut_post⟩ ← Std.Array.to_slice_mut.progress_spec
-
-    simp [Std.Array.to_slice_mut, Std.Array.to_slice] at slice_mut_post
-    obtain ⟨old_slice_post, new_slice_post⟩ := slice_mut_post
-
-    let* ⟨ s2, s2_len, s2_post ⟩ ← xor_long.spec
-    rw [old_slice_post] at s2_post
-    simp [s2_len] at s2_post
-
-    rw [slice_post] at s2_post
-    simp at s2_len
-    /- rw [s2_len] at s2_post -/ -- NOTE: Annoying that this doesn't work (setWidth's type depends on argument)
-
-    let* ⟨ s4, s4_post ⟩ ← keccak_p.spec
-    let* ⟨rest, rest_post ⟩ ← spec
-
-    simp [*]
-    apply congrArg
-    rw [absorb_def, absorb_def]
-    simp only [Array.foldl_extract]
-    rw [Array.foldl_step_right (l := i)]
-    case l_idx  | r_le | nontriv => (first | simp; done | simpa [n_val] using i_idx)
-    congr
-    ext idx idx_idx
-    simp [*]
-    rw [List.toBitVec] at s2_post
-    rw [←BitVec.getElem_ofBoolListLE, s2_post]
-    simp [Std.Array.from_slice, s2_post, old_slice_post, new_slice_post, ‹s2.length = 1600›']
-
-    rw [getElem_eq_getElem!,Array.getElem!_chunks_exact]
-    case i_idx | k_pos => (first | assumption | simpa [n_val] using i_idx)
-
-    simp
-  case isFalse i_oob =>
-    have := ‹bs.length / r.val - i.val = 0›'
-    simp [absorb, this, Array.foldl,Array.foldlM_start_stop (m := Id)]
-    rw [Array.extract_empty]
-    simp
-termination_by n.val - i.val
-decreasing_by scalar_decr_tac
-
-theorem Array.extract_start_stop(arr: Array α)
-(start_default : start = 0        := by omega)
-(stop_default :  stop  = arr.size := by omega)
-: arr.extract start stop = arr
-:= by subst start_default; subst stop_default; simp only [extract_size]
-
-@[progress]
-theorem algos.sponge_absorb_initial.spec
-  (bs : Std.Slice Bool) (r : Std.Usize) (s : Aeneas.Std.Array Bool 1600#usize)
-(r_pos: r.val > 0)
-: r.val < 1600
-→ s.val = List.replicate (Spec.b 6) false
-→ ∃ output,
-  sponge_absorb_initial bs r s = .ok output ∧
-  output.val = ListIR.absorb' ListIR.list_keccak_p s.val (bs.val.chunks_exact r)
-  -- ∧ output.val.toBitVec = ((absorb (s.val.toBitVec.cast (by simp; decide)) ((Array.mk bs.val).chunks_exact r)).cast (by simp; decide))
-:= by
-  intro r_lt s_zero
-  rw [sponge_absorb_initial]
-  let* ⟨ n, n_post ⟩ ← Std.Usize.div_spec
-  let* ⟨ res, res_post ⟩ ← algos.sponge_absorb_initial_loop.spec
-  simp [*, Array.extract_eq_self_of_le]
-
-  replace res_post := congrArg (f := BitVec.toList) res_post
-  simp at res_post
-  rw [res_post]
-
-  rw [Array.extract_start_stop (stop_default := by simp [*])]
-  rw [absorb.refinement]
-  simp [ListIR.absorb', s_zero]
-
-@[progress]
-theorem Aeneas.Std.core.slice.index.Slice.index_range_from_usize_spec(T: Type)
-(slice: Slice T)
-(i: ops.range.RangeFrom Usize)
-: i.start ≤ slice.length
-→ ∃ output,
-  Slice.index (Std.core.slice.index.SliceIndexRangeFromUsizeSlice T) slice i = .ok output ∧
-  output.val = slice.val.extract (start := i.start.val)
-:= by
-  intro inbound
-  simp only [index, SliceIndexRangeFromUsizeSlice.index]
-  simp_ifs
-  simp [Slice.drop]
-
--- @[simp]
--- def Aeneas.Std.UScalar.saturating_sub' {ty : UScalarTy} (x y : UScalar ty) : UScalar ty :=
---   UScalar.mk <| BitVec.ofFin ⟨x.val - y.val, Nat.lt_of_le_of_lt (Nat.sub_le _ _) x.bv.toFin.isLt⟩
-
--- @[simp]
--- theorem Aeneas.Std.UScalar.saturating_sub_def(a b: Std.UScalar ty)
--- : a.saturating_sub b = a.saturating_sub' b
--- := by
---   simp only [saturating_sub, BitVec.ofNat, Fin.ofNat', saturating_sub']
---   simp
---   rw [Nat.mod_eq_of_lt]
---   exact Nat.lt_of_le_of_lt (Nat.sub_le _ _) a.bv.toFin.isLt
-
--- /- attribute [scalar_tac_simps] Std.Array.to_slice -/
--- -- TODO: Me da el límite de recursión, no se por qué.
-
--- theorem Aeneas.Std.core.num.Usize.saturating_sub.spec(a b: Std.Usize)
--- : ∃ c, Std.toResult (saturating_sub a b) = .ok c ∧ c.val = a.val - b.val
--- := by
---   simp [saturating_sub, UScalar.saturating_sub', Std.toResult]
---   reduce
---   rfl
-
-
-@[progress]
-theorem algos.xor_long_at.spec'(a b: Std.Slice Bool)(offset: Std.Usize)
-: b.length + offset.val ≤ Std.Usize.max
-→ ∃ c,
-  xor_long_at a b offset = .ok c ∧
-  c.val = ListIR.xor_long_at a.val b.val offset.val
-:= by
-  intro nooverflow
-  let* ⟨ res, res_len, res_post ⟩ ← spec
-  ext i
-  · simp [res_len]
-  assume i_idx: i < res.length
-  case otherwise => simp_lists
-  rw [res_post, ListIR.getElem!_xor_long_at]
-  case a => assumption
-  simp [res_len] at i_idx
-  simp [i_idx]
-
-@[progress]
-theorem algos.xor_long.spec'(a b: Std.Slice Bool)
-: ∃ c,
-  xor_long a b = .ok c ∧
-  c.val = ListIR.xor_long a.val b.val
-:= by
-  rw [xor_long]
-  let* ⟨ res, post ⟩ ← xor_long_at.spec'
-  rw [post, ListIR.xor_long]
-
-
-/- set_option pp.coercions false in -/
-set_option maxHeartbeats 1000000 in
-@[progress]
-theorem algos.sponge_absorb_final.spec
-  (rest suffix : Std.Slice Bool) (r : Std.Usize) (s : Aeneas.Std.Array Bool _)
-: r.val ≥ 6
-→ rest.length < r
-→ suffix.length ≤ 4
-→ rest.length + suffix.length < Std.Usize.max
-→ ∃ output,
-  sponge_absorb_final s rest suffix r = .ok output ∧
-  output.val = sponge_absorb_final.panic_free ListIR.list_keccak_p r.val s.val rest.val suffix.val
-:= by
-  intro r_big_enough rest_lt suffix_le no_overflow
-  rw [sponge_absorb_final]
-
-  let* ⟨ old_s, mk_s1, old_s_post, new_s_post ⟩ ← Std.Array.to_slice_mut.spec'
-  let* ⟨ x1, x1_val ⟩ ← xor_long.spec'
-  -- ←Nat.sub_sub_eq_min
-  let* ⟨ nb_left, nb_left_post ⟩ ← Std.Usize.add_spec
-  simp at nb_left_post
-  split
-  case isTrue nb_left_ge_r =>
-    simp [nb_left_post] at nb_left_ge_r
-    let* ⟨ old_s1, mk_s2, old_s1_post, mk_s2_post ⟩ ← Std.Array.to_slice_mut.spec'
-    let* ⟨ i3, i3_post ⟩ ← Std.Usize.sub_spec'
-    simp at i3_post
-    let* ⟨ suffix_low, suffix_low_post ⟩ ← Std.core.slice.index.Slice.index.slice_index_range_usize_slice_spec
-    let* ⟨ x2, x2_val ⟩ ← xor_long_at.spec'
-    let* ⟨ x3, x3_val ⟩ ← keccak_p.spec'
-    let* ⟨ old_s2, mk_s3, old_s2_post, mk_s3_post ⟩ ← Std.Array.to_slice_mut.spec'
-    let* ⟨ suffix_high, suffix_high_post ⟩ ← Std.core.slice.index.Slice.index_range_from_usize_spec
-    let* ⟨ x4, x4_val ⟩ ← xor_long.spec'
-    let* ⟨ old_s3, mk_s4, old_s3_post, mk_s4_post ⟩ ← Std.Array.to_slice_mut.spec'
-    let* ⟨ single_one, single_one_post ⟩ ← Std.Array.to_slice.progress_spec
-    simp only [Std.toResult, Std.Array.make, Std.Array.to_slice] at single_one_post
-    let* ⟨ i7, i7_post ⟩ ← Std.Usize.sub_spec'
-    let* ⟨ x5, x5_val ⟩ ← xor_long_at.spec'
-    let* ⟨ old_s4, mk_s5,  old_s4_post, mk_s5_post ⟩ ← Std.Array.to_slice_mut.spec'
-    let* ⟨ i8, i8_post ⟩ ← Std.Usize.sub_spec'
-    let* ⟨ x6, x6_val ⟩ ← xor_long_at.spec'
-    let* ⟨ res, res_post_2 ⟩ ← keccak_p.spec'
-
-    simp [*, panic_free, Std.Array.from_slice, ListIR.xor_long]
-    simp_ifs
-    congr
-    simp_lists
-  case isFalse nb_left_idx =>
-    simp [nb_left_post] at nb_left_idx
-    let* ⟨ old_s1, mk_s2, old_s1_post, mk_s2_post ⟩ ← Std.Array.to_slice_mut.spec'
-    let* ⟨ s5, s5_val ⟩ ← xor_long_at.spec'
-    let* ⟨ _x_1, _x_2, _x_post_1, _x_post_2 ⟩ ← Std.Array.to_slice_mut.spec'
-    let* ⟨ single_one, single_one_post ⟩ ← Std.Array.to_slice.progress_spec
-    simp only [Std.toResult, Std.Array.make, Std.Array.to_slice] at single_one_post
-    let* ⟨ s9, s9_val ⟩ ← xor_long_at.spec'
-    let* ⟨ i3, i3_post ⟩ ← Std.Usize.add_spec
-    split
-    case isTrue nb_left_has_space =>
-      let* ⟨ _x_1, _x_2, _x_post_1, _x_post_2 ⟩ ← Std.Array.to_slice_mut.spec'
-      let* ⟨ i8, i8_post ⟩ ← Std.Usize.sub_spec'
-      let* ⟨ s19, s19_val ⟩ ← xor_long_at.spec'
-      let* ⟨ res, res_val ⟩ ← keccak_p.spec'
-
-      simp [*, panic_free, Std.Array.from_slice, ListIR.xor_long]
-      simp_ifs
-    case isFalse nb_left_has_space =>
-      let* ⟨ s11, s11_val ⟩ ← keccak_p.spec'
-      let* ⟨ _x_1, _x_2, _x_post_1, _x_post_2 ⟩ ← Std.Array.to_slice_mut.spec'
-      let* ⟨ i8, i8_post ⟩ ← Std.Usize.sub_spec'
-      let* ⟨ s19, s19_val ⟩ ← xor_long_at.spec'
-      let* ⟨ res, res_val ⟩ ← keccak_p.spec'
-
-      simp [*, panic_free, Std.Array.from_slice, ListIR.xor_long]
-      simp_ifs
-
-theorem List.chunks_exact_truncate{α: Type}(bs: List α)(r: Nat)
-: (bs.take (r*(bs.length/r))).chunks_exact r = bs.chunks_exact r
-:= by
-  assume r_pos: r > 0
-  case otherwise => simp at r_pos; subst r_pos; simp [List.chunks_exact]
-  have r_neZero: NeZero r := NeZero.of_pos r_pos
-  cases bs using List.cases_extract r
-  case onSmall small =>
-    unfold List.chunks_exact
-    simp [*]
-  case onBig chunk rest len_chunk =>
-    unfold List.chunks_exact
-    simp [*, r_neZero.out]
-    have: r <= r*(rest.length / r + 1) := by ring_nf; simp
-    have: rest.length / r + 1 = (chunk ++ rest).length / r := by simp [len_chunk, Nat.add_div_left, r_pos]
-    simp_lists [len_chunk]
-    simp +arith
-    ring_nf
-    simp +arith
-    apply List.chunks_exact_truncate
-termination_by bs.length
-decreasing_by simp [*]
-
-@[simp]
+@[simp, simp_lists_simps]
 theorem List.chunks_exact_nil(r: Nat): ([]: List α).chunks_exact r = [] := by unfold List.chunks_exact; simp
 
 theorem List.chunks_exact_split{α: Type}(bs: List α)(r: Nat)(i: Nat)
 : (bs.take (r*i)).chunks_exact r ++ (bs.drop (r*i)).chunks_exact r = bs.chunks_exact r
 := by
-  assume r_pos: r > 0
-  case otherwise => simp at r_pos; simp [r_pos]
+  assume r_pos: r > 0; case otherwise => simp at r_pos; simp [r_pos]
+  assume i_block_idx: r*i < bs.length; case otherwise => simp_lists
+  have   i_lt: i ≤ bs.length / r := by simp only [Nat.le_div_iff_mul_le r_pos, i_block_idx, le_of_lt, Nat.mul_comm i]
+  have   eq_len: ((bs.take (r*i)).chunks_exact r ++ (bs.drop (r*i)).chunks_exact r).length = (bs.chunks_exact r).length := by
+    simp [*, Nat.min_def, le_of_lt, Nat.add_assoc i, Nat.sub_div_mult_left]
 
-  ext j : 1
-  · simp
-    by_cases r*i ≥ bs.length
-    case pos h => simp [h]
-    case neg h =>
-      simp at h
-      have : i ≤ bs.length / r := by
-        simp only [Nat.le_div_iff_mul_le r_pos, h, le_of_lt, Nat.mul_comm i]
-      simp [h, le_of_lt, Nat.sub_div_mult_left, Nat.mul_div_cancel_left, r_pos, this]
-  assume h: r*i < bs.length
-  case otherwise =>
-    simp at h
-    rw [List.take_of_length_le h]
-    rw [List.drop_of_length_le h]
-    simp
-  have: i ≤ bs.length / r := by
-    simp only [Nat.le_div_iff_mul_le r_pos, h, le_of_lt, Nat.mul_comm i]
-  assume j < bs.length / r
-  case otherwise h =>
-    simp at h
-    rw [getElem!_neg]
-    rw [getElem!_neg]
-    · simp; omega
-    · simp [*, le_of_lt, Nat.sub_div_mult_left]
+  apply List.ext_getElem <;> simp [eq_len, ←getElem!_pos]
+  intro j j_idx
 
   by_cases j < i
   case pos j_lhs =>
-    rw [List.getElem!_append_left]
-    case h => simp [*, le_of_lt, Nat.mul_div_cancel, r_pos]
-    rw [List.getElem!_chunks_exact]
-    case a => simp [*, le_of_lt, Nat.mul_div_cancel, r_pos]
-    rw [List.getElem!_chunks_exact]
-    case a => simp; omega
+    rw [List.getElem!_append_left ]; case h => simp [*, le_of_lt]
+    rw [List.getElem!_chunks_exact]; case a => simp [*, le_of_lt]
+    rw [List.getElem!_chunks_exact]; case a => simp [*]
     simp
     rw [List.take_drop]
     rw [List.take_drop]
     rw [List.take_take]
     congr
-    ring_nf
-    simp
-    have : r*(j + 1) ≤ r*i := by
-      apply Nat.mul_le_mul_left
-      assumption
-    simpa [Nat.mul_add] using this
+    simp [‹r*j + r = r*(j + 1)›', Nat.add_one_le_of_lt j_lhs]
   case neg j_rhs =>
     simp at j_rhs
-    rw [List.getElem!_append_right]
-    case h => simp [*, le_of_lt]
-    rw [List.getElem!_chunks_exact]
-    case a => simp [*, le_of_lt, Nat.sub_div_mult_left]; omega
-    rw [List.getElem!_chunks_exact]
-    case a => simp [*]
+    rw [List.getElem!_append_right]; case h => simp [*, le_of_lt]
+    rw [List.getElem!_chunks_exact]; case a => simp [*, le_of_lt, Nat.sub_div_mult_left]; omega
+    rw [List.getElem!_chunks_exact]; case a => simp [*]
     simp [*, le_of_lt]
-    congr 1
-    · ring_nf; simp [Nat.mul_sub]
-    · congr
-      simp [Nat.mul_sub, *]
+    congr 2
+    simp [Nat.mul_sub, Nat.mul_le_mul_left r, j_rhs]
 
-
-/- @[progress] -/
-set_option maxRecDepth 1000000 in
-theorem algos.sponge_absorb.spec_list
-  (bs : Std.Slice Bool) (r : Std.Usize) [NeZero r.val](input : Aeneas.Std.Array Bool 1600#usize)
-  (suffix : Std.Slice Bool)
-: r.val ≥ 6
-→ r.val < 1600
-→ suffix.length ≤ 4
-→ input.val = List.replicate 1600 false
-→ let padding := (Spec.«pad10*1» r.val (bs.length % r.val + suffix.length)).toList
-∃ output,
-  sponge_absorb bs r input suffix = .ok output ∧
-  -- output.
-  -- output.val.toBitVec = (spec_sponge_absorb r.val (Nat.pos_of_neZero r.val) (bs.val.toArray ++ suffix.val.toArray)).cast (by simp [Spec.b, Spec.w])
-  -- absorb → absorb'
-  output.val =
-    ListIR.absorb' ListIR.list_keccak_p input.val (
-      (bs.val ++ suffix.val ++ padding).chunks_exact r
-    )
+theorem Spec.«size_pad10*1» (x m : Nat)
+: x > 0
+→ (Spec.«pad10*1» x m).size = (x - (m + 2) % x) % x + 2
 := by
-  intro r_big_enough r_bounded suffix_small input_zero
-  unfold sponge_absorb
-  have r_pos: r.val > 0 := by omega
+  intro x_pos
+  have: ((-m.cast -2) % x.cast).toNat = (x - (m + 2) % x) % x := by
+    zify
+    simp [Int.emod_nonneg, *, Nat.ne_zero_of_lt x_pos]
+    zmodify
+    simp
+  simp [Spec.«pad10*1», this]
+  simp +arith
 
-  let* ⟨ s1, s1_post ⟩ ← sponge_absorb_initial.spec
-  let* ⟨ n, n_post ⟩ ← Std.Usize.div_spec
-  have := Nat.mul_div_le bs.length r
-  let* ⟨ i1, i1_post ⟩ ← Std.Usize.mul_spec
-  let* ⟨ rest, rest_post ⟩ ← Std.core.slice.index.Slice.index_range_from_usize_spec
-  have rest_len: rest.length < r := by simp [*, ←Nat.mod_eq_sub, Nat.mod_lt]
-  let* ⟨ res, res_post ⟩ ← sponge_absorb_final.spec
+theorem Spec.«pad10*1_mod» (x m : Nat)
+: (Spec.«pad10*1» x (m % x)) = (Spec.«pad10*1» x m)
+:= by simp [«pad10*1»]; congr 4; zmodify
 
-  simp only [*]
-  rw [ref.interesting_part_of_the_proof.proof]
-  case a =>
-    simp [ref.interesting_part_of_the_proof.preconditions, *, ←Nat.mod_eq_sub, Nat.mod_lt]
-  simp [-List.reduceReplicate, ←Nat.mod_eq_sub, Nat.mod_lt]
-  generalize (Spec.«pad10*1» r.val (bs.length % r.val + suffix.length)).toList = padding
-  rw [ListIR.absorb'_absorb']
-  congr
-  rw [List.take_of_length_le (h := by simp [Nat.add_comm (bs.length % r), Nat.div_add_mod])]
+theorem Spec.«size_pad10*1_eq_ite» (x m : Nat)
+: x > 2
+→ (Spec.«pad10*1» x m).size = if m%x = x - 1 then 1 + x else x - m % x
+:= by
+  intro x_gt
+  have x_pos: x > 0 := by omega
+  rw [←Spec.«pad10*1_mod»]
+  generalize m'_def: m % x = m'
+  have m'_lt: m' < x := by simp [←m'_def, Nat.mod_lt, x_pos]
+  simp [Spec.«size_pad10*1», x_pos]
+  split
+  · simp +arith [*, ‹1 < x›', le_of_lt, ←Nat.sub_add_comm, Nat.mod_eq_of_lt]
+  · if m' = x - 2 then
+      simp +arith [*, ‹1 < x›', le_of_lt, ←Nat.sub_add_comm, Nat.mod_eq_of_lt]
+      omega
+    else
+      simp [*, ‹m' + 2 < x›', le_of_lt,  Nat.mod_eq_of_lt, ←Nat.sub_add_comm]
 
-  rw [←List.chunks_exact_truncate]
+theorem Spec.«pad10*1_of_mtpl_8»(r bs_len: Nat)
+: r > 0
+→ (Spec.«pad10*1» (8*r) (8*bs_len)).size = 8*(r - (bs_len % r))
+:= by
+  intro r_pos
+  rw [←Spec.«pad10*1_mod»]
+  generalize r'_def: 8*r = r'
+  have: r' > 0 := by omega
+  have: r' > 2 := by omega
+  generalize bs_len'_def: (8 * bs_len) % r' = bs_len'
+  simp [←r'_def, Nat.mul_mod_mul_left] at bs_len'_def
+  have bs_len'_lt: bs_len' < r' := by simp [←r'_def, ←bs_len'_def, Nat.mod_lt, r_pos]
 
-  rw [←List.append_assoc]
-  rw [←List.drop_append_of_le_length (by scalar_tac)]
-  rw [←List.drop_append_of_le_length (by trans bs.length <;> (first | assumption | simp))]
-  rw [←List.take_append_of_le_length (l₂ := suffix.val) (by assumption)]
-  rw [←List.take_append_of_le_length (l₂ := padding) (by trans bs.length <;> (first | assumption | simp))]
-  rw [List.chunks_exact_split, List.append_assoc]
+  simp [Spec.«size_pad10*1_eq_ite», this, Nat.mul_mod_mul_right, Nat.mod_eq_of_lt, bs_len'_lt]
+  split <;> simp [*, Nat.mul_sub]
+  omega
+
+-- set_option maxHeartbeats 1000000 in
+-- set_option maxRecDepth 1000000 in
+-- theorem algos.sponge_absorb.spec
+--   (bs : Std.Slice Std.U8) (r : Std.Usize) (s : algos.StateArray) (extra : Std.U8)
+--   (r_pos: 0 < 8*r.val)
+--   (r_bnd: 8*r.val < Spec.b 6)
+-- : 8 ∣ r.val
+-- /- The following condition is needed because `extra` contains both the suffix (either for
+--    SHA3 or SHAKE) and the first bit of padding. We must be able to separate them for the spec
+--    to make sense. -/
+-- → (∃ i < 5, extra.toBits[i]! = true ∧ ∀ j ≥ i, extra.toBits[j]! = false)
+-- → s.toBits = List.replicate (Spec.b 6) false
+-- →  ∃ output extra_idx, -- TODO: Move extra_idx to somewhere it makes more sense.
+--   sponge_absorb bs r s extra = .ok output ∧
+--   output.toBits = (Spec.sponge.absorb (f := Spec.Keccak.P 6 24) (pad := Spec.«pad10*1») ⟨8*r.val, ⟨r_pos, r_bnd⟩⟩ ⟨bs.toBits ++ extra.toBits.take extra_idx⟩).toList
+-- := by
+--   -- Preconditions
+--   intro r_mtpl_8 ⟨extra_idx, extra_idx_lt, getElem_extra_idx, getElem_gt_extra_idx⟩ s_eq_zero
+--   have last_extra_eq_false: extra.toBits[7]! = false := by apply getElem_gt_extra_idx; omega
+--   have extra_idx_le_8: extra_idx ≤ 8 := by omega
+--   have: 0 < r.val := by omega
+
+--   -- Progress
+--   unfold sponge_absorb
+--   simp [Std.core.slice.index.Slice.index]
+--   progress* by simp [*, Nat.mul_div_self_eq_mod_sub_self]; scalar_tac
+--   exists extra_idx
+--   simp [*, Std.Array.toBits, Std.Slice.toBits]
+--   simp only [*, IR.absorb.unfold, IR.array_absorb.refinement, IR.absorb.refinement, ‹0 < r.val›', List.size_toArray]
+
+--   -- Definitions
+--   generalize padding_def: Spec.«pad10*1» (8*r.val) _ = padding
+--   have size_padding: padding.size = 8*r.val - (8*(bs.length% r)) - extra_idx := by
+--     simp [*, ←padding_def, ←Nat.mul_comm 8, extra_idx_lt]
+--     rw [Spec.«size_pad10*1_eq_ite»]
+--     split
+--     · sorry
+
+
+--   simp [Array.toList_chunks_exact]
+--   congr
+--   simp [←Nat.mod_eq_sub]
+--   conv => rhs; rw [←List.chunks_exact_split _ _ (i := (bs.length / r))]
+--   rw [List.take_append_of_le_length]; swap; { simp [←Nat.mul_comm 8, Nat.mul_assoc, Nat.mul_div_le] }
+--   conv => lhs; enter [1]; rw [←List.chunks_exact_truncate]
+--   simp [←Nat.mul_comm 8, Nat.mul_div_mul_left]
+
+--   rw [List.drop_append_of_le_length]; swap; { simp [←Nat.mul_comm 8, Nat.mul_assoc, Nat.mul_div_le]}
+--   simp [Nat.mul_assoc]
+--   generalize rest_def: List.drop (8 * (r.val * (bs.length / r.val))) bs.toBits = rest
+--   have len_rest_padding: (rest ++ padding.toList).length = 8*r := by
+--     have := (le_of_lt (Nat.mod_lt _ ‹0 < r.val›):bs.length % r.val ≤ r.val)
+--     simp [size_padding, ←rest_def]
+--     simp [size_padding, ←Nat.mul_comm 8, Nat.mul_assoc, ←Nat.mul_add, ←Nat.mul_sub, Nat.mul_lt_mul_left (by decide: 0 < 8)]
+--     rw [←Nat.mod_eq_sub]
+--     rw [←Nat.add_sub_assoc this, Nat.add_comm, Nat.add_sub_cancel]
+
+--   unfold List.chunks_exact
+--   simp [len_rest_padding, ‹r.val ≠ 0›', List.take_of_length_le]
+
+  -- apply List.ext_getElem
+  -- · simp [-List.length_append, ←Nat.mul_comm 8, Nat.mul_div_mul_left, Spec.«size_pad10*1»]
+  --   simp
+  -- rw [←List.chunks_exact_split (i := bs.length / r)]
+  -- simp
+
+  -- unfold List.chunks_exact
+  -- simp
+  -- simp_ifs
+  -- apply List.ext_getElem <;> simp [←getElem!_pos, ←Nat.mul_comm 8, Nat.mul_div_mul_left]
+  -- -- TODO: Now we have these two cases, one were bs.length = 8*r * length_bs'
+  sorry
+
+
+
+
+-- theorem Spec.«pad10*1_length» (x m : Nat)
+-- : (Spec.«pad10*1» x m).size = (2 + (-(m + 2: Int) % x).toNat)
+-- := by simp +arith [«pad10*1», neg_add, -neg_add_rev, -Int.reduceNeg]
+
+-- def spec_sponge (r: Nat)(r_pos: r > 0):=
+--   have: NeZero r := ⟨Nat.ne_zero_of_lt r_pos⟩
+--   Spec.sponge (f := Spec.Keccak.P 6 24) (pad := Spec.«pad10*1»)
+-- def spec_sponge_absorb (r: Nat)(r_pos: r > 0) :=
+--   have: NeZero r := ⟨Nat.ne_zero_of_lt r_pos⟩
+--   Spec.sponge.absorb (f := Spec.Keccak.P 6 24) (pad := Spec.«pad10*1») (r := r)
+-- def spec_sponge_squeze{m d}(r: Nat)(r_pos: r > 0) :=
+--   have: NeZero r := ⟨Nat.ne_zero_of_lt r_pos⟩
+--   Spec.sponge.squeeze (m := m) (d := d) (f := Spec.Keccak.P 6 24) (r := r)
+
+-- /- #check BitVec.setWidth_cast -/
+
+-- def absorb.upd(S: BitVec (Spec.b 6))(P: Vector Bool r): BitVec (Spec.b 6) :=
+--   Spec.Keccak.P 6 24 (S ^^^ (BitVec.ofBoolListLE <| P.toList).setWidth (Spec.b 6))
+
+-- def absorb{r: Nat}(S: BitVec (Spec.b 6))(Ps: Array (Vector Bool r)) := Id.run do
+--   let mut S := S
+--   for P in Ps do
+--     S := absorb.upd S P
+--   return S
+
+-- def algos.sponge_absorb_final.panic_free
+--   (keccak_p: List Bool → List Bool)
+--   (r: Nat)
+--   (s rest suffix: List Bool)
+-- : List Bool
+-- := Id.run do
+--   let mut s := s
+--   s := ListIR.xor_long s rest
+--   let nb_left := rest.length + suffix.length
+--   if nb_left >= r then
+--     s := ListIR.xor_long_at s (suffix.take (r - rest.length)) rest.length
+--   -- if nb_left >= r then
+--     s := keccak_p s
+--     s := ListIR.xor_long s (suffix.drop (r - rest.length))
+--     s := ListIR.xor_long_at s [true] (rest.length + suffix.length - r)
+--     s := ListIR.xor_long_at s [true] (r-1)
+--   else
+--     s := ListIR.xor_long_at s suffix rest.length
+--     s := ListIR.xor_long_at s [true] nb_left
+--     if nb_left + 1 < r then
+--       s := ListIR.xor_long_at s [true] (r-1)
+--     else
+--       s := keccak_p s
+--       s := ListIR.xor_long_at s [true] (r-1)
+--   keccak_p s
+
+
+-- @[scalar_tac_simps]
+-- theorem Nat.sub_div_self(a b: Nat)
+-- :(a - b) / b = a / b - 1 := by
+--   by_cases b > 0
+--   case neg h => simp at h; subst h; simp
+--   by_cases a >= b
+--   case pos h =>
+--     have: a = (a - b) + b := (Nat.sub_eq_iff_eq_add h).mp rfl
+--     rw [this, Nat.add_sub_cancel, Nat.add_div_right, Nat.add_sub_cancel]
+--     assumption
+--   case neg h =>
+--     simp at h
+--     simp [Nat.div_eq_of_lt h, Nat.sub_eq_zero_of_le (le_of_lt h)]
+
+-- @[scalar_tac_simps]
+-- theorem Nat.sub_div_mult_left(a b: Nat)
+-- :(a - b*i) / b = a / b - i := by
+--   by_cases b > 0
+--   case neg h => simp at h; subst h; simp
+--   case pos =>
+--     cases i
+--     case zero => simp
+--     case succ i' =>
+--       simp [Nat.mul_add, Nat.sub_add_eq, Nat.sub_div_self]
+--       rw [Nat.sub_div_mult_left]
+
+-- theorem BitVec.cast_xor(bv bv2: BitVec n)(eq: n = m)
+-- : (bv ^^^ bv2).cast eq = bv.cast eq ^^^ bv2.cast eq
+-- := by ext i i_lt; simp
+
+-- attribute [simp] Aeneas.Std.core.slice.index.Slice.index
+
+
+-- private theorem List.foldl_congr{ls ls': List α}
+-- : ls = ls'
+-- → upd = upd'
+-- → init = init'
+-- → ls.foldl upd init = ls'.foldl upd' init'
+-- := by rintro rfl rfl rfl; rfl
+
+-- set_option maxRecDepth 1000000 in
+-- set_option maxHeartbeats 1000000 in
+-- theorem absorb.refinement(r: Nat)(S: BitVec (Spec.b 6))(bs: Array Bool)
+-- : (absorb S (bs.chunks_exact r)).toList = ListIR.absorb' ListIR.list_keccak_p S.toList (bs.toList.chunks_exact r)
+-- := by
+--   unfold absorb ListIR.absorb'
+--   simp [ListIR.list_keccak_p, ListIR.xor_long.def, -Array.size_chunks_exact]
+--   rw [←Array.foldl_toList]
+--   rw [Array.chunks_exact, List.chunks_exact]
+--   split <;> simp_ifs
+--   case isTrue h =>
+--     simp
+--     ext i
+--     · simp [Spec.b, Spec.w]
+--     by_cases i < 1600 <;> simp
+--     case pos h => intros; assumption
+--     case neg h =>
+--       rw [getElem!_neg]
+--       case h => simpa using h
+--       simp
+--   case isFalse h =>
+--     simp
+--     generalize_proofs _ len_extract
+--     have ih := absorb.refinement r (@upd r S ⟨bs.extract 0 r, len_extract⟩) (bs.extract r)
+--     simp [absorb,ListIR.absorb', ListIR.list_keccak_p, ListIR.xor_long.def] at ih
+--     rw [ih]
+--     rw [List.foldl_congr]
+--     · rw [List.take_of_length_le]
+--       simp
+--     · ext s chunk
+--       · simp
+--       simp
+--     · rw [upd]
+--       simp [List.setWidth, Spec.b, Spec.w]
+--       rw [List.take_of_length_le (by simp)]
+--       apply congrArg
+--       apply congrArg
+--       ext i i_idx
+--       rw [ListIR.xor_long, ListIR.xor_long_at]
+--       simp at i_idx
+--       simp [←Bool.default_bool,←List.getElem!_eq_getElem?_getD, i_idx]
+--       have: S.toList.length = 1600 := by simp [Spec.b, Spec.w]
+--       if h: i < r then
+--         simp_lists
+--         rw [List.getElem!_zipWith]
+--         case a => simp [*]
+--         case a => simp [*]; omega
+--         simp [getElem_eq_getElem!, *]
+--       else
+--         simp_lists
+--         simp at h
+--         simp +arith [getElem_eq_getElem!, ←Nat.add_sub_assoc, h]
+-- termination_by bs.size
+
+-- abbrev ref.interesting_part_of_the_proof.preconditions(r: Nat)(s rest suffix: List Bool) :=
+--   r ≥ 6 -- Otherwise, we don't have suffix + 2 ≤ r
+-- ∧ suffix.length ≤ 4 -- Taken from the actual uses of `suffix` in SHA3
+-- ∧   rest.length < r -- Since rest is what's left after absorb_initial
+-- ∧ s.length = 1600 -- The state has length Spec.b 6
+
+-- set_option maxRecDepth 100000000 in
+-- set_option maxHeartbeats 1000000 in
+-- theorem ref.interesting_part_of_the_proof.case1{r: Nat}{s rest suffix: List Bool}
+--   (hyp: (rest ++ suffix).length ≥ r)
+-- : preconditions r s rest suffix
+-- → let padding := (Spec.«pad10*1» r (rest.length + suffix.length)).toList
+--   (rest ++ suffix ++ padding).chunks_exact r = [(rest ++ suffix).take r, (suffix.drop (r - rest.length) ++ padding)]
+-- := by
+--   /-
+--   · (rest ++ suffix) >= r
+--     Then we have
+--      (rest ++ suffix ++ padding).chunks_exact k =
+--      = [(rest ++ suffix).take r, (suffix.drop (r - rest.length) ++ padding)]
+--   -/
+--   rintro ⟨r_big_enough,suffix_len_le,rest_len_lt,len_s⟩ padding
+--   have len_padding: (Spec.«pad10*1» r (rest.length + suffix.length)).size = 2*r - (rest.length + suffix.length) := by
+--     simp [Spec.«pad10*1_length», -neg_add_rev]
+--     have := mod_manipulation (h1 := r_big_enough) (h2 := rest_len_lt) (h3 := suffix_len_le) (h4 := by scalar_tac)
+--     rw [this]
+--     scalar_tac
+--   have len_append: (rest.length + suffix.length + padding.length) = 2*r := by
+--     simp [padding, len_padding]
+--     scalar_tac
+--   simp at hyp
+--   have len_chunks: ((rest ++ suffix ++ padding).chunks_exact r).length = 2 := by
+--     simp
+--     rw [←Nat.add_assoc, len_append, Nat.mul_div_cancel]
+--     omega
+
+--   -- Execute List.chunks_exact
+--   unfold List.chunks_exact
+--   simp_ifs
+--   unfold List.chunks_exact
+--   simp_ifs
+--   unfold List.chunks_exact
+--   simp_ifs
+
+--   congr 1
+--   · ext i
+--     · simp [←Nat.add_assoc, len_append]
+--       omega
+--     by_cases i < r
+--     case neg => simp_lists
+--     rw [List.getElem!_take_append_beg]
+--     case pos.x => assumption
+--     case pos.x => simp; omega
+--     simp_lists
+--   · congr
+--     ext i
+--     · simp [←Nat.add_assoc, len_append]
+--       omega
+--     simp_lists
+--     congr
+--     omega
+
+-- set_option maxRecDepth 100000000 in
+-- set_option maxHeartbeats 1000000 in
+-- theorem ref.interesting_part_of_the_proof.case2{r: Nat}{s rest suffix: List Bool}
+--   (hyp: (rest ++ suffix).length = r-1)
+-- : preconditions r s rest suffix
+-- → let padding := (Spec.«pad10*1» r (rest.length + suffix.length)).toList
+--   (rest ++ suffix ++ padding).chunks_exact r = [rest ++ suffix ++ [true], List.replicate (r-1) false ++ [true]]
+-- := by
+--   /-
+--   · (rest ++ suffix) = r - 1
+--     Then we have
+--      (rest ++ suffix ++ padding).chunks_exact k =
+--      = [rest ++ suffix ++ [true], List.replicate false (r-1) ++ [true]]
+--   -/
+--   rintro ⟨r_big_enough,suffix_len_le,rest_len_lt,len_s⟩ padding
+--   have len_padding: (Spec.«pad10*1» r (rest.length + suffix.length)).size = 2*r - (rest.length + suffix.length) := by
+--     simp at hyp
+--     simp [Spec.«pad10*1_length», -neg_add_rev, hyp, r_big_enough]
+--     zify
+--     rw [Nat.cast_sub (by omega)]
+--     rw [Nat.cast_sub (by omega)]
+--     rw [Nat.cast_sub (by omega)]
+--     rw [Nat.cast_mul]
+--     ring_nf
+--     simp [Int.neg_emod_eq_sub_emod]
+--     rw [
+--       Int.emod_eq_of_lt (H1:=by omega) (H2:=by omega),
+--       Int.max_eq_left (by omega)
+--     ]
+--     omega
+--   have len_append: (rest.length + suffix.length + padding.length) = 2*r := by
+--     simp [padding, len_padding]; scalar_tac
+
+--   simp at hyp
+--   have len_chunks: ((rest ++ suffix ++ padding).chunks_exact r).length = 2 := by
+--     simp
+--     rw [←Nat.add_assoc, len_append, Nat.mul_div_cancel]
+--     omega
+
+--   -- Execute List.chunks_exact
+--   unfold List.chunks_exact
+--   simp_ifs
+--   unfold List.chunks_exact
+--   simp_ifs
+--   unfold List.chunks_exact
+--   simp_ifs
+--   congr
+--   · ext i
+--     · simp; scalar_tac
+--     simp_lists
+--     congr
+--     simp [hyp, Nat.sub_sub_self, ‹r >= 1›', List.take_one, List.head?, padding, Spec.«pad10*1», BitVec.toList]
+--   · ext i
+--     · simp; scalar_tac
+--     simp_lists
+--     simp [hyp] at len_padding
+--     simp [hyp, Nat.sub_sub_self, ‹r >= 1›', padding, Array.getElem!_toList, getElem!_padding, len_padding,
+--        -Bool.if_false_right, -Bool.if_false_left, -Bool.if_true_left] -- Keep `if`s for `simp_ifs` to process
+--     by_cases i = r -1
+--     case pos h => simp_ifs [h]; simp
+--     case neg =>
+--       simp_ifs
+--       by_cases i > r - 1
+--       case neg => simp_ifs
+--       case pos =>
+--         simp_ifs
+--         rw [getElem!_neg]
+--         simp
+--         scalar_tac
+
+-- set_option maxRecDepth 100000000 in
+-- set_option maxHeartbeats 1000000 in
+-- theorem ref.interesting_part_of_the_proof.case3{r: Nat}{s rest suffix: List Bool}
+--   (hyp: (rest ++ suffix).length <= r-2)
+-- : preconditions r s rest suffix
+-- → let padding := (Spec.«pad10*1» r (rest.length + suffix.length)).toList
+--   (rest ++ suffix ++ padding).chunks_exact r = [rest ++ suffix ++ [true] ++ List.replicate (r -2 - rest.length - suffix.length) false ++ [true]]
+-- := by
+--   /-
+--   · (rest ++ suffix) <= r - 2
+--     Then we have
+--      (rest ++ suffix ++ padding).chunks_exact k =
+--      = [rest ++ suffix ++ [true, true]]
+--   -/
+--   rintro ⟨r_big_enough,suffix_len_le,rest_len_lt,len_s⟩ padding
+--   have len_padding: (Spec.«pad10*1» r (rest.length + suffix.length)).size = r - (rest.length + suffix.length) := by
+--     simp at hyp
+--     simp [Spec.«pad10*1_length», -neg_add_rev]
+--     zify
+--     rw [Nat.cast_sub (by omega),
+--         Int.neg_emod_eq_sub_emod,
+--         Int.emod_eq_of_lt (H1:=by omega) (H2:=by omega)]
+--     simp
+--     rw [Int.max_eq_left (by omega)]
+--     omega
+--   have len_append: (rest.length + suffix.length + padding.length) = r := by
+--     simp [padding, len_padding]
+--     scalar_tac
+--   have len_chunks: ((rest ++ suffix ++ padding).chunks_exact r).length = 1 := by
+--     simp [←Nat.add_assoc, len_append, Nat.div_self, ‹r > 0›']
+
+--   unfold List.chunks_exact
+--   simp_ifs
+
+--   unfold List.chunks_exact
+--   simp_ifs
+--   simp
+--   ext i
+--   · simp; scalar_tac
+--   simp_lists
+--   congr
+--   simp [padding, Spec.«pad10*1», BitVec.toList]
+--   have := Spec.«pad10*1_length» r (rest.length + suffix.length)
+--   simp at this
+--   ring_nf at this ⊢
+--   scalar_tac
+
+-- set_option maxHeartbeats 1000000 in
+-- theorem ref.interesting_part_of_the_proof.proof(r: Nat)(s rest suffix: List Bool)
+-- : preconditions r s rest suffix
+-- → let f := ListIR.list_keccak_p
+--   let padding := (Spec.«pad10*1» r (rest.length + suffix.length)).toList
+--   algos.sponge_absorb_final.panic_free f r s rest suffix =
+--     ListIR.absorb' f s (
+--       (rest ++ suffix ++ padding).chunks_exact r
+--     )
+-- := by
+--   rintro precond f padding
+--   have ⟨r_big_enough,suffix_len_le,rest_len_lt,len_s⟩ := precond
+--   /-
+--   There are three cases we must consider:
+--   · (rest ++ suffix) >= r
+--     Then we have
+--      (rest ++ suffix ++ padding).chunks_exact k =
+--      = [(rest ++ suffix).take r, (suffix.drop (r - rest.length) ++ padding)]
+--   · (rest ++ suffix) = r - 1
+--     Then we have
+--      (rest ++ suffix ++ padding).chunks_exact k =
+--      = [rest ++ suffix ++ [true], List.replicate false (r-1) ++ [true]]
+--   · (rest ++ suffix) <= r - 2
+--     Then we have
+--      (rest ++ suffix ++ padding).chunks_exact k =
+--      = [rest ++ suffix ++ [true, true]]
+--   -/
+--   if      cond1: (rest ++ suffix).length ≥ r then
+--     rw [case1 cond1 precond]
+--     simp at cond1
+--     simp [ListIR.absorb', algos.sponge_absorb_final.panic_free, *, ListIR.xor_long]
+
+--     generalize leftover_val: (rest.length + suffix.length - r) = leftover
+--     rw [ListIR.xor_long_at_twice_separate]
+--     case compatible_offset => scalar_tac
+
+--     rw [ListIR.xor_long_at_twice_separate]
+--     case compatible_offset => scalar_tac
+
+--     rw [ListIR.xor_long_at_twice_separate]
+--     case compatible_offset => scalar_tac
+
+--     congr
+--     · simp +arith [List.take_append_of_ge_length, le_of_lt rest_len_lt]
+--     · simp +arith; scalar_tac
+--     · have padding_len
+--       : (Spec.«pad10*1» r (rest.length + suffix.length)).size = 2 * r - rest.length - suffix.length
+--       := by
+--         simp [Spec.«pad10*1»]
+--         have: (2: Int) = (2: Nat).cast := by congr
+--         rw [this]
+--         have(a b: Int): a - b = a + -b := by exact rfl
+--         rw [this]
+--         simp only [←Nat.cast_sub, ←neg_add, Nat.cast_add]
+--         conv =>
+--           lhs
+--           rhs
+--           rw [Nat.cast_ofNat]
+--           conv => enter [1, 1, 1, 1, 1]; rw [Int.add_comm]
+--           rw [mod_manipulation (h1 := r_big_enough) (h2 := rest_len_lt) (h3 := suffix_len_le) (h4 := cond1)]
+--         scalar_tac
+
+--       ext i
+--       · simp [padding_len]
+--         scalar_tac
+--       conv => rhs; rw [Array.getElem!_toList]
+--       simp [getElem!_padding, -List.cons_append, -List.singleton_append, -List.cons_append_fun]
+--       by_cases h: i = 0
+--       case pos => simp [h]
+--       by_cases h: i = (Spec.«pad10*1» r (rest.length + suffix.length)).size - 1
+--       -- by_cases h: i = 2* r - rest.length - suffix.length - 1
+--       case pos =>
+--         rw [List.getElem!_append_right]
+--         case h => scalar_tac
+--         rw [List.getElem!_append_right]
+--         case h => scalar_tac
+--         simp [h, padding_len, ←leftover_val]
+--         rw [List.getElem!_singleton]
+--         scalar_tac
+--       by_cases h: i < (Spec.«pad10*1» r (rest.length + suffix.length)).size
+--       case neg =>
+--         rw [getElem!_neg]
+--         case h => simp [Spec.«pad10*1»] at *; scalar_tac
+--         simp [Spec.«pad10*1»] at *
+--         simp [*]
+--       case pos =>
+--         rw [getElem!_pos]
+--         case h => simp [padding_len] at *; scalar_tac
+--         rw [List.getElem_append_right]
+--         case h₁ => scalar_tac
+--         rw [List.getElem_append_left]
+--         case h => scalar_tac
+--         simp [padding_len] at *; simp [*]
+--         scalar_tac
+
+--   else if cond2: (rest ++ suffix).length = r - 1 then
+--     rw [case2 cond2 precond]
+--     replace cond2 := ‹r = (rest ++ suffix).length + 1›'
+--     simp [ListIR.absorb', algos.sponge_absorb_final.panic_free, *, ListIR.xor_long]
+
+--     rw [ListIR.xor_long_at_twice_separate]
+--     case compatible_offset => scalar_tac
+
+--     rw [ListIR.xor_long_at_twice_separate]
+--     case compatible_offset => scalar_tac
+
+--     simp [ListIR.xor_long_of_xor_long_at]
+--     congr
+--     -- have{α: Type}(x ls: List α): (x ++ ls) = ls ↔ x = [] := by exact?
+--     simp_lists
+--     scalar_tac
+
+--   else if cond3: (rest ++ suffix).length ≤ r - 2 then
+--     rw [case3 cond3 precond]
+--     simp at cond3
+--     simp [ListIR.absorb', algos.sponge_absorb_final.panic_free, *, ListIR.xor_long]
+--     simp_ifs
+
+--     rw [ListIR.xor_long_at_twice_separate]
+--     case compatible_offset => scalar_tac
+
+--     rw [ListIR.xor_long_at_twice_separate]
+--     case compatible_offset => scalar_tac
+
+--     rw [ListIR.xor_long_at_twice_separate]
+--     case compatible_offset => scalar_tac
+
+--     simp only [ListIR.xor_long_of_xor_long_at]
+--     congr
+--     · simp
+--     · rw [List.append_right_eq_self, List.replicate_eq_nil_iff]
+--       -- scalar_tac -- TODO: Gives maxRecDepth error
+--       omega
+--     · simp only [List.length_singleton, Nat.sub_add_eq]
+--       congr
+
+--   else omega -- Absurd
+
+-- theorem absorb_def{r: Nat}(S: BitVec (Spec.b 6))(Ps: Array (Vector Bool r))
+-- : absorb S Ps = Ps.foldl (absorb.upd · ·) S
+-- := by simp [absorb]
+
+-- theorem absorb.spec (N : Array Spec.Bit) (r: Nat)(r_pos: r > 0)
+-- : spec_sponge_absorb r r_pos N = absorb (0#(Spec.b 6)) ((N ++ Spec.«pad10*1» r N.size).chunks_exact r)
+-- := by
+--   rw [spec_sponge_absorb, Spec.sponge.absorb, absorb]
+--   -- NOTE: I needed to exercise a bit too much control here.
+--   simp [←Array.foldl_toList,-Array.size_chunks_exact, -Array.size_map, upd]
+
+-- @[progress]
+-- theorem Aeneas.Std.Array.to_slice_mut.spec{α : Type u} {n : Usize} (a : Array α n)
+-- : ∃ old new,
+--   Std.toResult (a.to_slice_mut) = .ok (old, new) ∧
+--   old = a.to_slice ∧
+--   new = a.from_slice
+-- := by simp [to_slice_mut, Std.toResult]
+
+-- attribute [simp] Std.Slice
+-- set_option maxHeartbeats 1000000 in
+-- @[progress]
+-- theorem algos.sponge_absorb_initial_loop.spec
+--   (bs : Std.Slice Bool) (r : Std.Usize) (s : Aeneas.Std.Array Bool 1600#usize) (n i : Std.Usize)
+-- : n.val = bs.length / r.val
+-- → (r_pos: r.val > 0)
+-- → i.val ≤ n.val
+-- → r.val < 1600
+-- → ∃ output,
+--   sponge_absorb_initial_loop bs r s n i = .ok output ∧
+--   output.val.toBitVec = (
+--     (
+--       absorb (s.val.toBitVec.cast (by simp [Spec.w, Spec.b])) (bs.val.toArray.chunks_exact r |>.drop i)
+--     ).cast (by simp [Spec.w, Spec.b])
+--   )
+-- := by
+--   rintro n_val r_pos i_idx r_le
+--   rw [sponge_absorb_initial_loop]
+--   split
+--   case isTrue i_idx =>
+--      -- r * i < r * n = r * (bs.length / r) ≤ bs.length ≤ Usize.max
+--     have _: r.val*i.val ≤ bs.length := le_of_lt $ calc r.val * i.val
+--         _ < r.val * n := Nat.mul_lt_mul_of_pos_left i_idx r_pos
+--         _ = r.val * (bs.length / r) := by simp [n_val]
+--         _ ≤ bs.length := Nat.mul_div_le bs.length ↑r
+
+--      -- r * (i + 1) ≤ r * n = r * (bs.length / r) ≤ bs.length ≤ Usize.max
+--     have _: r.val*(i.val + 1) ≤ bs.length := calc r.val * (i.val + 1)
+--         _ ≤ r.val * n := Nat.mul_le_mul_left r.val i_idx
+--         _ = r.val * (bs.length / r) := by simp [n_val]
+--         _ ≤ bs.length := Nat.mul_div_le bs.length ↑r
+
+--     let* ⟨ i1, i1_post ⟩ ← Std.Usize.mul_spec
+--     let* ⟨ i2, i2_post ⟩ ← Std.Usize.add_spec
+--     let* ⟨ i3, i3_post ⟩ ← Std.Usize.mul_spec
+--     let* ⟨ slice, slice_post ⟩ ← Std.core.slice.index.Slice.index.slice_index_range_usize_slice_spec
+--     fsimp only [*] at slice_post
+--     let* ⟨old_slice, new_slice, slice_mut_post⟩ ← Std.Array.to_slice_mut.progress_spec
+
+--     simp [Std.Array.to_slice_mut, Std.Array.to_slice] at slice_mut_post
+--     obtain ⟨old_slice_post, new_slice_post⟩ := slice_mut_post
+
+--     let* ⟨ s2, s2_len, s2_post ⟩ ← xor_long.spec
+--     rw [old_slice_post] at s2_post
+--     simp [s2_len] at s2_post
+
+--     rw [slice_post] at s2_post
+--     simp at s2_len
+--     /- rw [s2_len] at s2_post -/ -- NOTE: Annoying that this doesn't work (setWidth's type depends on argument)
+
+--     let* ⟨ s4, s4_post ⟩ ← keccak_p.spec
+--     let* ⟨rest, rest_post ⟩ ← spec
+
+--     simp [*]
+--     apply congrArg
+--     rw [absorb_def, absorb_def]
+--     simp only [Array.foldl_extract]
+--     rw [Array.foldl_step_right (l := i)]
+--     case l_idx  | r_le | nontriv => (first | simp; done | simpa [n_val] using i_idx)
+--     congr
+--     ext idx idx_idx
+--     simp [*]
+--     rw [List.toBitVec] at s2_post
+--     rw [←BitVec.getElem_ofBoolListLE, s2_post]
+--     simp [Std.Array.from_slice, s2_post, old_slice_post, new_slice_post, ‹s2.length = 1600›']
+
+--     rw [getElem_eq_getElem!,Array.getElem!_chunks_exact]
+--     case i_idx | k_pos => (first | assumption | simpa [n_val] using i_idx)
+
+--     simp
+--   case isFalse i_oob =>
+--     have := ‹bs.length / r.val - i.val = 0›'
+--     simp [absorb, this, Array.foldl,Array.foldlM_start_stop (m := Id)]
+--     rw [Array.extract_empty]
+--     simp
+-- termination_by n.val - i.val
+-- decreasing_by scalar_decr_tac
+
+-- theorem Array.extract_start_stop(arr: Array α)
+-- (start_default : start = 0        := by omega)
+-- (stop_default :  stop  = arr.size := by omega)
+-- : arr.extract start stop = arr
+-- := by subst start_default; subst stop_default; simp only [extract_size]
+
+-- @[progress]
+-- theorem algos.sponge_absorb_initial.spec
+--   (bs : Std.Slice Bool) (r : Std.Usize) (s : Aeneas.Std.Array Bool 1600#usize)
+-- (r_pos: r.val > 0)
+-- : r.val < 1600
+-- → s.val = List.replicate (Spec.b 6) false
+-- → ∃ output,
+--   sponge_absorb_initial bs r s = .ok output ∧
+--   output.val = ListIR.absorb' ListIR.list_keccak_p s.val (bs.val.chunks_exact r)
+--   -- ∧ output.val.toBitVec = ((absorb (s.val.toBitVec.cast (by simp; decide)) ((Array.mk bs.val).chunks_exact r)).cast (by simp; decide))
+-- := by
+--   intro r_lt s_zero
+--   rw [sponge_absorb_initial]
+--   let* ⟨ n, n_post ⟩ ← Std.Usize.div_spec
+--   let* ⟨ res, res_post ⟩ ← algos.sponge_absorb_initial_loop.spec
+--   simp [*, Array.extract_eq_self_of_le]
+
+--   replace res_post := congrArg (f := BitVec.toList) res_post
+--   simp at res_post
+--   rw [res_post]
+
+--   rw [Array.extract_start_stop (stop_default := by simp [*])]
+--   rw [absorb.refinement]
+--   simp [ListIR.absorb', s_zero]
+
+-- @[progress]
+-- theorem Aeneas.Std.core.slice.index.Slice.index_range_from_usize_spec(T: Type)
+-- (slice: Slice T)
+-- (i: ops.range.RangeFrom Usize)
+-- : i.start ≤ slice.length
+-- → ∃ output,
+--   Slice.index (Std.core.slice.index.SliceIndexRangeFromUsizeSlice T) slice i = .ok output ∧
+--   output.val = slice.val.extract (start := i.start.val)
+-- := by
+--   intro inbound
+--   simp only [index, SliceIndexRangeFromUsizeSlice.index]
+--   simp_ifs
+--   simp [Slice.drop]
+
+-- -- @[simp]
+-- -- def Aeneas.Std.UScalar.saturating_sub' {ty : UScalarTy} (x y : UScalar ty) : UScalar ty :=
+-- --   UScalar.mk <| BitVec.ofFin ⟨x.val - y.val, Nat.lt_of_le_of_lt (Nat.sub_le _ _) x.bv.toFin.isLt⟩
+
+-- -- @[simp]
+-- -- theorem Aeneas.Std.UScalar.saturating_sub_def(a b: Std.UScalar ty)
+-- -- : a.saturating_sub b = a.saturating_sub' b
+-- -- := by
+-- --   simp only [saturating_sub, BitVec.ofNat, Fin.ofNat', saturating_sub']
+-- --   simp
+-- --   rw [Nat.mod_eq_of_lt]
+-- --   exact Nat.lt_of_le_of_lt (Nat.sub_le _ _) a.bv.toFin.isLt
+
+-- -- /- attribute [scalar_tac_simps] Std.Array.to_slice -/
+-- -- -- TODO: Me da el límite de recursión, no se por qué.
+
+-- -- theorem Aeneas.Std.core.num.Usize.saturating_sub.spec(a b: Std.Usize)
+-- -- : ∃ c, Std.toResult (saturating_sub a b) = .ok c ∧ c.val = a.val - b.val
+-- -- := by
+-- --   simp [saturating_sub, UScalar.saturating_sub', Std.toResult]
+-- --   reduce
+-- --   rfl
+
+
+-- @[progress]
+-- theorem algos.xor_long_at.spec'(a b: Std.Slice Bool)(offset: Std.Usize)
+-- : b.length + offset.val ≤ Std.Usize.max
+-- → ∃ c,
+--   xor_long_at a b offset = .ok c ∧
+--   c.val = ListIR.xor_long_at a.val b.val offset.val
+-- := by
+--   intro nooverflow
+--   let* ⟨ res, res_len, res_post ⟩ ← spec
+--   ext i
+--   · simp [res_len]
+--   assume i_idx: i < res.length
+--   case otherwise => simp_lists
+--   rw [res_post, ListIR.getElem!_xor_long_at]
+--   case a => assumption
+--   simp [res_len] at i_idx
+--   simp [i_idx]
+
+-- @[progress]
+-- theorem algos.xor_long.spec'(a b: Std.Slice Bool)
+-- : ∃ c,
+--   xor_long a b = .ok c ∧
+--   c.val = ListIR.xor_long a.val b.val
+-- := by
+--   rw [xor_long]
+--   let* ⟨ res, post ⟩ ← xor_long_at.spec'
+--   rw [post, ListIR.xor_long]
+
+
+-- /- set_option pp.coercions false in -/
+-- set_option maxHeartbeats 1000000 in
+-- @[progress]
+-- theorem algos.sponge_absorb_final.spec
+--   (rest suffix : Std.Slice Bool) (r : Std.Usize) (s : Aeneas.Std.Array Bool _)
+-- : r.val ≥ 6
+-- → rest.length < r
+-- → suffix.length ≤ 4
+-- → rest.length + suffix.length < Std.Usize.max
+-- → ∃ output,
+--   sponge_absorb_final s rest suffix r = .ok output ∧
+--   output.val = sponge_absorb_final.panic_free ListIR.list_keccak_p r.val s.val rest.val suffix.val
+-- := by
+--   intro r_big_enough rest_lt suffix_le no_overflow
+--   rw [sponge_absorb_final]
+
+--   let* ⟨ old_s, mk_s1, old_s_post, new_s_post ⟩ ← Std.Array.to_slice_mut.spec'
+--   let* ⟨ x1, x1_val ⟩ ← xor_long.spec'
+--   -- ←Nat.sub_sub_eq_min
+--   let* ⟨ nb_left, nb_left_post ⟩ ← Std.Usize.add_spec
+--   simp at nb_left_post
+--   split
+--   case isTrue nb_left_ge_r =>
+--     simp [nb_left_post] at nb_left_ge_r
+--     let* ⟨ old_s1, mk_s2, old_s1_post, mk_s2_post ⟩ ← Std.Array.to_slice_mut.spec'
+--     let* ⟨ i3, i3_post ⟩ ← Std.Usize.sub_spec'
+--     simp at i3_post
+--     let* ⟨ suffix_low, suffix_low_post ⟩ ← Std.core.slice.index.Slice.index.slice_index_range_usize_slice_spec
+--     let* ⟨ x2, x2_val ⟩ ← xor_long_at.spec'
+--     let* ⟨ x3, x3_val ⟩ ← keccak_p.spec'
+--     let* ⟨ old_s2, mk_s3, old_s2_post, mk_s3_post ⟩ ← Std.Array.to_slice_mut.spec'
+--     let* ⟨ suffix_high, suffix_high_post ⟩ ← Std.core.slice.index.Slice.index_range_from_usize_spec
+--     let* ⟨ x4, x4_val ⟩ ← xor_long.spec'
+--     let* ⟨ old_s3, mk_s4, old_s3_post, mk_s4_post ⟩ ← Std.Array.to_slice_mut.spec'
+--     let* ⟨ single_one, single_one_post ⟩ ← Std.Array.to_slice.progress_spec
+--     simp only [Std.toResult, Std.Array.make, Std.Array.to_slice] at single_one_post
+--     let* ⟨ i7, i7_post ⟩ ← Std.Usize.sub_spec'
+--     let* ⟨ x5, x5_val ⟩ ← xor_long_at.spec'
+--     let* ⟨ old_s4, mk_s5,  old_s4_post, mk_s5_post ⟩ ← Std.Array.to_slice_mut.spec'
+--     let* ⟨ i8, i8_post ⟩ ← Std.Usize.sub_spec'
+--     let* ⟨ x6, x6_val ⟩ ← xor_long_at.spec'
+--     let* ⟨ res, res_post_2 ⟩ ← keccak_p.spec'
+
+--     simp [*, panic_free, Std.Array.from_slice, ListIR.xor_long]
+--     simp_ifs
+--     congr
+--     simp_lists
+--   case isFalse nb_left_idx =>
+--     simp [nb_left_post] at nb_left_idx
+--     let* ⟨ old_s1, mk_s2, old_s1_post, mk_s2_post ⟩ ← Std.Array.to_slice_mut.spec'
+--     let* ⟨ s5, s5_val ⟩ ← xor_long_at.spec'
+--     let* ⟨ _x_1, _x_2, _x_post_1, _x_post_2 ⟩ ← Std.Array.to_slice_mut.spec'
+--     let* ⟨ single_one, single_one_post ⟩ ← Std.Array.to_slice.progress_spec
+--     simp only [Std.toResult, Std.Array.make, Std.Array.to_slice] at single_one_post
+--     let* ⟨ s9, s9_val ⟩ ← xor_long_at.spec'
+--     let* ⟨ i3, i3_post ⟩ ← Std.Usize.add_spec
+--     split
+--     case isTrue nb_left_has_space =>
+--       let* ⟨ _x_1, _x_2, _x_post_1, _x_post_2 ⟩ ← Std.Array.to_slice_mut.spec'
+--       let* ⟨ i8, i8_post ⟩ ← Std.Usize.sub_spec'
+--       let* ⟨ s19, s19_val ⟩ ← xor_long_at.spec'
+--       let* ⟨ res, res_val ⟩ ← keccak_p.spec'
+
+--       simp [*, panic_free, Std.Array.from_slice, ListIR.xor_long]
+--       simp_ifs
+--     case isFalse nb_left_has_space =>
+--       let* ⟨ s11, s11_val ⟩ ← keccak_p.spec'
+--       let* ⟨ _x_1, _x_2, _x_post_1, _x_post_2 ⟩ ← Std.Array.to_slice_mut.spec'
+--       let* ⟨ i8, i8_post ⟩ ← Std.Usize.sub_spec'
+--       let* ⟨ s19, s19_val ⟩ ← xor_long_at.spec'
+--       let* ⟨ res, res_val ⟩ ← keccak_p.spec'
+
+--       simp [*, panic_free, Std.Array.from_slice, ListIR.xor_long]
+--       simp_ifs
+
+-- theorem List.chunks_exact_truncate{α: Type}(bs: List α)(r: Nat)
+-- : (bs.take (r*(bs.length/r))).chunks_exact r = bs.chunks_exact r
+-- := by
+--   assume r_pos: r > 0
+--   case otherwise => simp at r_pos; subst r_pos; simp [List.chunks_exact]
+--   have r_neZero: NeZero r := NeZero.of_pos r_pos
+--   cases bs using List.cases_extract r
+--   case onSmall small =>
+--     unfold List.chunks_exact
+--     simp [*]
+--   case onBig chunk rest len_chunk =>
+--     unfold List.chunks_exact
+--     simp [*, r_neZero.out]
+--     have: r <= r*(rest.length / r + 1) := by ring_nf; simp
+--     have: rest.length / r + 1 = (chunk ++ rest).length / r := by simp [len_chunk, Nat.add_div_left, r_pos]
+--     simp_lists [len_chunk]
+--     simp +arith
+--     ring_nf
+--     simp +arith
+--     apply List.chunks_exact_truncate
+-- termination_by bs.length
+-- decreasing_by simp [*]
+
+-- @[simp]
+-- theorem List.chunks_exact_nil(r: Nat): ([]: List α).chunks_exact r = [] := by unfold List.chunks_exact; simp
+
+-- theorem List.chunks_exact_split{α: Type}(bs: List α)(r: Nat)(i: Nat)
+-- : (bs.take (r*i)).chunks_exact r ++ (bs.drop (r*i)).chunks_exact r = bs.chunks_exact r
+-- := by
+--   assume r_pos: r > 0
+--   case otherwise => simp at r_pos; simp [r_pos]
+
+--   ext j : 1
+--   · simp
+--     by_cases r*i ≥ bs.length
+--     case pos h => simp [h]
+--     case neg h =>
+--       simp at h
+--       have : i ≤ bs.length / r := by
+--         simp only [Nat.le_div_iff_mul_le r_pos, h, le_of_lt, Nat.mul_comm i]
+--       simp [h, le_of_lt, Nat.sub_div_mult_left, Nat.mul_div_cancel_left, r_pos, this]
+--   assume h: r*i < bs.length
+--   case otherwise =>
+--     simp at h
+--     rw [List.take_of_length_le h]
+--     rw [List.drop_of_length_le h]
+--     simp
+--   have: i ≤ bs.length / r := by
+--     simp only [Nat.le_div_iff_mul_le r_pos, h, le_of_lt, Nat.mul_comm i]
+--   assume j < bs.length / r
+--   case otherwise h =>
+--     simp at h
+--     rw [getElem!_neg]
+--     rw [getElem!_neg]
+--     · simp; omega
+--     · simp [*, le_of_lt, Nat.sub_div_mult_left]
+
+--   by_cases j < i
+--   case pos j_lhs =>
+--     rw [List.getElem!_append_left]
+--     case h => simp [*, le_of_lt, Nat.mul_div_cancel, r_pos]
+--     rw [List.getElem!_chunks_exact]
+--     case a => simp [*, le_of_lt, Nat.mul_div_cancel, r_pos]
+--     rw [List.getElem!_chunks_exact]
+--     case a => simp; omega
+--     simp
+--     rw [List.take_drop]
+--     rw [List.take_drop]
+--     rw [List.take_take]
+--     congr
+--     ring_nf
+--     simp
+--     have : r*(j + 1) ≤ r*i := by
+--       apply Nat.mul_le_mul_left
+--       assumption
+--     simpa [Nat.mul_add] using this
+--   case neg j_rhs =>
+--     simp at j_rhs
+--     rw [List.getElem!_append_right]
+--     case h => simp [*, le_of_lt]
+--     rw [List.getElem!_chunks_exact]
+--     case a => simp [*, le_of_lt, Nat.sub_div_mult_left]; omega
+--     rw [List.getElem!_chunks_exact]
+--     case a => simp [*]
+--     simp [*, le_of_lt]
+--     congr 1
+--     · ring_nf; simp [Nat.mul_sub]
+--     · congr
+--       simp [Nat.mul_sub, *]
+
+
+-- /- @[progress] -/
+-- set_option maxRecDepth 1000000 in
+-- theorem algos.sponge_absorb.spec_list
+--   (bs : Std.Slice Bool) (r : Std.Usize) [NeZero r.val](input : Aeneas.Std.Array Bool 1600#usize)
+--   (suffix : Std.Slice Bool)
+-- : r.val ≥ 6
+-- → r.val < 1600
+-- → suffix.length ≤ 4
+-- → input.val = List.replicate 1600 false
+-- → let padding := (Spec.«pad10*1» r.val (bs.length % r.val + suffix.length)).toList
+-- ∃ output,
+--   sponge_absorb bs r input suffix = .ok output ∧
+--   -- output.
+--   -- output.val.toBitVec = (spec_sponge_absorb r.val (Nat.pos_of_neZero r.val) (bs.val.toArray ++ suffix.val.toArray)).cast (by simp [Spec.b, Spec.w])
+--   -- absorb → absorb'
+--   output.val =
+--     ListIR.absorb' ListIR.list_keccak_p input.val (
+--       (bs.val ++ suffix.val ++ padding).chunks_exact r
+--     )
+-- := by
+--   intro r_big_enough r_bounded suffix_small input_zero
+--   unfold sponge_absorb
+--   have r_pos: r.val > 0 := by omega
+
+--   let* ⟨ s1, s1_post ⟩ ← sponge_absorb_initial.spec
+--   let* ⟨ n, n_post ⟩ ← Std.Usize.div_spec
+--   have := Nat.mul_div_le bs.length r
+--   let* ⟨ i1, i1_post ⟩ ← Std.Usize.mul_spec
+--   let* ⟨ rest, rest_post ⟩ ← Std.core.slice.index.Slice.index_range_from_usize_spec
+--   have rest_len: rest.length < r := by simp [*, ←Nat.mod_eq_sub, Nat.mod_lt]
+--   let* ⟨ res, res_post ⟩ ← sponge_absorb_final.spec
+
+--   simp only [*]
+--   rw [ref.interesting_part_of_the_proof.proof]
+--   case a =>
+--     simp [ref.interesting_part_of_the_proof.preconditions, *, ←Nat.mod_eq_sub, Nat.mod_lt]
+--   simp [-List.reduceReplicate, ←Nat.mod_eq_sub, Nat.mod_lt]
+--   generalize (Spec.«pad10*1» r.val (bs.length % r.val + suffix.length)).toList = padding
+--   rw [ListIR.absorb'_absorb']
+--   congr
+--   rw [List.take_of_length_le (h := by simp [Nat.add_comm (bs.length % r), Nat.div_add_mod])]
+
+--   rw [←List.chunks_exact_truncate]
+
+--   rw [←List.append_assoc]
+--   rw [←List.drop_append_of_le_length (by scalar_tac)]
+--   rw [←List.drop_append_of_le_length (by trans bs.length <;> (first | assumption | simp))]
+--   rw [←List.take_append_of_le_length (l₂ := suffix.val) (by assumption)]
+--   rw [←List.take_append_of_le_length (l₂ := padding) (by trans bs.length <;> (first | assumption | simp))]
+--   rw [List.chunks_exact_split, List.append_assoc]
